Adjust recursor code to deal with bound free positions

operations/VVSubst.thy
@@ -1,5 +1,5 @@
 theory VVSubst
-  imports "./Fixpoint"
+  imports "./Least_Fixpoint"
 begin
 
 (********************************)
@@ -18,14 +18,14 @@ abbreviation validP :: "('var, 'tyvar, 'a, 'b, 'c) P \<Rightarrow> bool" where
     |supp f1| <o |UNIV::'var set| \<and> |supp f2| <o |UNIV::'tyvar set| \<and>
     |supp f3| <o |UNIV::'a set|"
 
-definition U1ctor :: "('var::{var_T1_pre, var_T2_pre}, 'tyvar::{var_T1_pre, var_T2_pre}, 'a::{var_T1_pre, var_T2_pre}, 'b, 'var, 'tyvar, ('var, 'tyvar, 'a, 'b, 'c) rec_T1, ('var, 'tyvar, 'a, 'b, 'c) rec_T1, ('var, 'tyvar, 'a, 'b, 'c) rec_T2, ('var, 'tyvar, 'a, 'b, 'c) rec_T2) T1_pre \<Rightarrow> ('var, 'tyvar, 'a, 'b, 'c) P \<Rightarrow> ('var, 'tyvar, 'a, 'c) U1" where
+definition U1ctor :: "('var::{var_T1_pre, var_T2_pre}, 'tyvar::{var_T1_pre, var_T2_pre}, 'a::{var_T1_pre, var_T2_pre}, 'b, 'var, 'tyvar, 'var, ('var, 'tyvar, 'a, 'b, 'c) rec_T1, ('var, 'tyvar, 'a, 'b, 'c) rec_T1, ('var, 'tyvar, 'a, 'b, 'c) rec_T2, ('var, 'tyvar, 'a, 'b, 'c) rec_T2) T1_pre \<Rightarrow> ('var, 'tyvar, 'a, 'b, 'c) P \<Rightarrow> ('var, 'tyvar, 'a, 'c) U1" where
   "U1ctor x p \<equiv> case p of (f1, f2, f3, f4) \<Rightarrow>
-    T1_ctor (map_T1_pre f1 f2 f3 f4 id id
+    T1_ctor (map_T1_pre f1 f2 f3 f4 id id f1
       ((\<lambda>R. R p) \<circ> snd) ((\<lambda>R. R p) \<circ> snd) ((\<lambda>R. R p) \<circ> snd) ((\<lambda>R. R p) \<circ> snd) x
   )"
-definition U2ctor :: "('var::{var_T1_pre, var_T2_pre}, 'tyvar::{var_T1_pre, var_T2_pre}, 'a::{var_T1_pre, var_T2_pre}, 'b, 'var, 'tyvar, ('var, 'tyvar, 'a, 'b, 'c) rec_T1, ('var, 'tyvar, 'a, 'b, 'c) rec_T1, ('var, 'tyvar, 'a, 'b, 'c) rec_T2, ('var, 'tyvar, 'a, 'b, 'c) rec_T2) T2_pre \<Rightarrow> ('var, 'tyvar, 'a, 'b, 'c) P \<Rightarrow> ('var, 'tyvar, 'a, 'c) U2" where
+definition U2ctor :: "('var::{var_T1_pre, var_T2_pre}, 'tyvar::{var_T1_pre, var_T2_pre}, 'a::{var_T1_pre, var_T2_pre}, 'b, 'var, 'tyvar, 'var, ('var, 'tyvar, 'a, 'b, 'c) rec_T1, ('var, 'tyvar, 'a, 'b, 'c) rec_T1, ('var, 'tyvar, 'a, 'b, 'c) rec_T2, ('var, 'tyvar, 'a, 'b, 'c) rec_T2) T2_pre \<Rightarrow> ('var, 'tyvar, 'a, 'b, 'c) P \<Rightarrow> ('var, 'tyvar, 'a, 'c) U2" where
   "U2ctor x p \<equiv> case p of (f1, f2, f3, f4) \<Rightarrow>
-    T2_ctor (map_T2_pre f1 f2 f3 f4 id id
+    T2_ctor (map_T2_pre f1 f2 f3 f4 id id f1
       ((\<lambda>R. R p) \<circ> snd) ((\<lambda>R. R p) \<circ> snd) ((\<lambda>R. R p) \<circ> snd) ((\<lambda>R. R p) \<circ> snd) x
   )"
 
@@ -38,23 +38,23 @@ abbreviation Pmap :: "('var \<Rightarrow> 'var) \<Rightarrow> ('tyvar \<Rightarr
   "Pmap g1 g2 p \<equiv> case p of (f1, f2, f3, f4) \<Rightarrow> (compSS g1 f1, compSS g2 f2, f3, f4)"
 
 abbreviation U1map :: "('var::{var_T1_pre, var_T2_pre} \<Rightarrow> 'var) \<Rightarrow> ('tyvar::{var_T1_pre, var_T2_pre} \<Rightarrow> 'tyvar) \<Rightarrow> ('var, 'tyvar, 'a::{var_T1_pre, var_T2_pre}, 'b) T1 \<Rightarrow> ('var, 'tyvar, 'a, 'c) U1 \<Rightarrow> ('var, 'tyvar, 'a, 'c) U1" where
-  "U1map f1 f2 t \<equiv> \<lambda>u. rrename_T1 f1 f2 u"
+  "U1map f1 f2 t \<equiv> \<lambda>u. permute_T1 f1 f2 u"
 abbreviation U2map :: "('var::{var_T1_pre, var_T2_pre} \<Rightarrow> 'var) \<Rightarrow> ('tyvar::{var_T1_pre, var_T2_pre} \<Rightarrow> 'tyvar) \<Rightarrow> ('var, 'tyvar, 'a::{var_T1_pre, var_T2_pre}, 'b) T2 \<Rightarrow> ('var, 'tyvar, 'a, 'c) U2 \<Rightarrow> ('var, 'tyvar, 'a, 'c) U2" where
-  "U2map f1 f2 t \<equiv> \<lambda>u. rrename_T2 f1 f2 u"
+  "U2map f1 f2 t \<equiv> \<lambda>u. permute_T2 f1 f2 u"
 
 abbreviation U1FVars_1 :: "('var, 'tyvar, 'a, 'b) T1 \<Rightarrow> ('var::{var_T1_pre, var_T2_pre}, 'tyvar::{var_T1_pre, var_T2_pre}, 'a::{var_T1_pre, var_T2_pre}, 'c) U1 \<Rightarrow> 'var set" where
-  "U1FVars_1 t u \<equiv> FFVars_T11 u"
+  "U1FVars_1 t u \<equiv> FVars_T11 u"
 abbreviation U1FVars_2 :: "('var, 'tyvar, 'a, 'b) T1 \<Rightarrow> ('var::{var_T1_pre, var_T2_pre}, 'tyvar::{var_T1_pre, var_T2_pre}, 'a::{var_T1_pre, var_T2_pre}, 'c) U1 \<Rightarrow> 'tyvar set" where
-  "U1FVars_2 t u \<equiv> FFVars_T12 u"
+  "U1FVars_2 t u \<equiv> FVars_T12 u"
 abbreviation U2FVars_1 :: "('var, 'tyvar, 'a, 'b) T2 \<Rightarrow> ('var::{var_T1_pre, var_T2_pre}, 'tyvar::{var_T1_pre, var_T2_pre}, 'a::{var_T1_pre, var_T2_pre}, 'c) U2 \<Rightarrow> 'var set" where
-  "U2FVars_1 t u \<equiv> FFVars_T21 u"
+  "U2FVars_1 t u \<equiv> FVars_T21 u"
 abbreviation U2FVars_2 :: "('var, 'tyvar, 'a, 'b) T2 \<Rightarrow> ('var::{var_T1_pre, var_T2_pre}, 'tyvar::{var_T1_pre, var_T2_pre}, 'a::{var_T1_pre, var_T2_pre}, 'c) U2 \<Rightarrow> 'tyvar set" where
-  "U2FVars_2 t u \<equiv> FFVars_T22 u"
+  "U2FVars_2 t u \<equiv> FVars_T22 u"
 
 function set3_raw_T1 :: "('var::{var_T1_pre,var_T2_pre}, 'tyvar::{var_T1_pre,var_T2_pre}, 'a::{var_T1_pre,var_T2_pre}, 'b) raw_T1 \<Rightarrow> 'a set"
   and set3_raw_T2 :: "('var::{var_T1_pre,var_T2_pre}, 'tyvar::{var_T1_pre,var_T2_pre}, 'a::{var_T1_pre,var_T2_pre}, 'b) raw_T2 \<Rightarrow> 'a set" where
-  "set3_raw_T1 (raw_T1_ctor x) = set3_T1_pre x \<union> \<Union>(set3_raw_T1 ` set7_T1_pre x) \<union> \<Union>(set3_raw_T1 ` set8_T1_pre x)  \<union> \<Union>(set3_raw_T2 ` set9_T1_pre x) \<union> \<Union>(set3_raw_T2 ` set10_T1_pre x)"
-| "set3_raw_T2 (raw_T2_ctor x) = set3_T2_pre x \<union> \<Union>(set3_raw_T1 ` set7_T2_pre x) \<union> \<Union>(set3_raw_T1 ` set8_T2_pre x)  \<union> \<Union>(set3_raw_T2 ` set9_T2_pre x) \<union> \<Union>(set3_raw_T2 ` set10_T2_pre x)"
+  "set3_raw_T1 (raw_T1_ctor x) = set3_T1_pre x \<union> \<Union>(set3_raw_T1 ` set8_T1_pre x) \<union> \<Union>(set3_raw_T1 ` set9_T1_pre x)  \<union> \<Union>(set3_raw_T2 ` set10_T1_pre x) \<union> \<Union>(set3_raw_T2 ` set11_T1_pre x)"
+| "set3_raw_T2 (raw_T2_ctor x) = set3_T2_pre x \<union> \<Union>(set3_raw_T1 ` set8_T2_pre x) \<union> \<Union>(set3_raw_T1 ` set9_T2_pre x)  \<union> \<Union>(set3_raw_T2 ` set10_T2_pre x) \<union> \<Union>(set3_raw_T2 ` set11_T2_pre x)"
      apply pat_completeness
     apply (unfold sum.inject raw_T1.inject raw_T2.inject sum.distinct)
     apply ((hypsubst, rule refl) | erule sum.distinct[THEN notE])+
@@ -64,14 +64,14 @@ termination
     Inl t1 \<Rightarrow> (case y of Inl t1' \<Rightarrow> subshape_T1_T1 t1 t1' | Inr t2 \<Rightarrow> subshape_T1_T2 t1 t2)
   | Inr t2 \<Rightarrow> (case y of Inl t1 \<Rightarrow> subshape_T2_T1 t2 t1 | Inr t2' \<Rightarrow> subshape_T2_T2 t2 t2')
  }")
-          apply (rule T1.wf_subshape)
+          apply (rule wf_subshape)
          apply (unfold mem_Collect_eq prod.case sum.case)
-         apply (erule T1.set_subshapes)+
+         apply (erule set_subshapess)+
   done
 function set4_raw_T1 :: "('var::{var_T1_pre,var_T2_pre}, 'tyvar::{var_T1_pre,var_T2_pre}, 'a::{var_T1_pre,var_T2_pre}, 'b) raw_T1 \<Rightarrow> 'b set"
   and set4_raw_T2 :: "('var::{var_T1_pre,var_T2_pre}, 'tyvar::{var_T1_pre,var_T2_pre}, 'a::{var_T1_pre,var_T2_pre}, 'b) raw_T2 \<Rightarrow> 'b set" where
-  "set4_raw_T1 (raw_T1_ctor x) = set4_T1_pre x \<union> \<Union>(set4_raw_T1 ` set7_T1_pre x) \<union> \<Union>(set4_raw_T1 ` set8_T1_pre x)  \<union> \<Union>(set4_raw_T2 ` set9_T1_pre x) \<union> \<Union>(set4_raw_T2 ` set10_T1_pre x)"
-| "set4_raw_T2 (raw_T2_ctor x) = set4_T2_pre x \<union> \<Union>(set4_raw_T1 ` set7_T2_pre x) \<union> \<Union>(set4_raw_T1 ` set8_T2_pre x)  \<union> \<Union>(set4_raw_T2 ` set9_T2_pre x) \<union> \<Union>(set4_raw_T2 ` set10_T2_pre x)"
+  "set4_raw_T1 (raw_T1_ctor x) = set4_T1_pre x \<union> \<Union>(set4_raw_T1 ` set8_T1_pre x) \<union> \<Union>(set4_raw_T1 ` set9_T1_pre x)  \<union> \<Union>(set4_raw_T2 ` set10_T1_pre x) \<union> \<Union>(set4_raw_T2 ` set11_T1_pre x)"
+| "set4_raw_T2 (raw_T2_ctor x) = set4_T2_pre x \<union> \<Union>(set4_raw_T1 ` set8_T2_pre x) \<union> \<Union>(set4_raw_T1 ` set9_T2_pre x)  \<union> \<Union>(set4_raw_T2 ` set10_T2_pre x) \<union> \<Union>(set4_raw_T2 ` set11_T2_pre x)"
      apply pat_completeness
     apply (unfold sum.inject raw_T1.inject raw_T2.inject)
     apply ((hypsubst, rule refl) | erule sum.distinct[THEN notE])+
@@ -81,9 +81,9 @@ termination
     Inl t1 \<Rightarrow> (case y of Inl t1' \<Rightarrow> subshape_T1_T1 t1 t1' | Inr t2 \<Rightarrow> subshape_T1_T2 t1 t2)
   | Inr t2 \<Rightarrow> (case y of Inl t1 \<Rightarrow> subshape_T2_T1 t2 t1 | Inr t2' \<Rightarrow> subshape_T2_T2 t2 t2')
  }")
-          apply (rule T1.wf_subshape)
+          apply (rule wf_subshape)
          apply (unfold mem_Collect_eq prod.case sum.case)
-         apply (erule T1.set_subshapes)+
+         apply (erule set_subshapess)+
   done
 
 definition "set3_T1 x \<equiv> set3_raw_T1 (quot_type.rep Rep_T1 x)"
@@ -94,13 +94,13 @@ definition "set4_T2 x \<equiv> set4_raw_T2 (quot_type.rep Rep_T2 x)"
 
 coinductive rel_T1 :: "('b \<Rightarrow> 'c \<Rightarrow> bool) \<Rightarrow> ('var::{var_T1_pre,var_T2_pre}, 'tyvar::{var_T1_pre,var_T2_pre}, 'a::{var_T1_pre,var_T2_pre}, 'b) T1 \<Rightarrow> ('var, 'tyvar, 'a, 'c) T1 \<Rightarrow> bool"
   and rel_T2 :: "('b \<Rightarrow> 'c \<Rightarrow> bool) \<Rightarrow> ('var, 'tyvar, 'a, 'b) T2 \<Rightarrow> ('var, 'tyvar, 'a, 'c) T2 \<Rightarrow> bool" where
-  "\<lbrakk> bij f1 ; |supp f1| <o |UNIV::'var set| ; id_on ((\<Union>(FFVars_T11 ` set8_T1_pre x) - set5_T1_pre x) \<union> (\<Union>(FFVars_T21 ` set10_T1_pre x) - set5_T1_pre x)) f1 ;
-     bij f2 ; |supp f2| <o |UNIV::'tyvar set| ; id_on (\<Union>(FFVars_T12 ` set8_T1_pre x) - set6_T1_pre x) f2 ;
-    rel_T1_pre R (rel_T1 R) (rel_T1 R) (rel_T2 R) (rel_T2 R) (map_T1_pre id id id id f1 f2 id (rrename_T1 f1 f2) id (rrename_T2 f1 id) x) y \<rbrakk>
+  "\<lbrakk> bij f1 ; |supp f1| <o |UNIV::'var set| ; id_on ((set7_T1_pre x \<union> \<Union>(FVars_T11 ` set9_T1_pre x) \<union> \<Union>(FVars_T21 ` set11_T1_pre x)) - set5_T1_pre x) f1 ;
+     bij f2 ; |supp f2| <o |UNIV::'tyvar set| ; id_on (\<Union>(FVars_T12 ` set9_T1_pre x) - set6_T1_pre x) f2 ;
+    rel_T1_pre R (rel_T1 R) (rel_T1 R) (rel_T2 R) (rel_T2 R) (map_T1_pre id id id id f1 f2 f1 id (permute_T1 f1 f2) id (permute_T2 f1 id) x) y \<rbrakk>
     \<Longrightarrow> rel_T1 R (T1_ctor x) (T1_ctor y)"
-| "\<lbrakk> bij f1 ; |supp f1| <o |UNIV::'var set| ; id_on ((\<Union>(FFVars_T11 ` set8_T2_pre x2) - set5_T2_pre x2) \<union> (\<Union>(FFVars_T21 ` set10_T2_pre x2) - set5_T2_pre x2)) f1 ;
-     bij f2 ; |supp f2| <o |UNIV::'tyvar set| ; id_on (\<Union>(FFVars_T12 ` set8_T2_pre x2) - set6_T2_pre x2) f2 ;
-    rel_T2_pre R (rel_T1 R) (rel_T1 R) (rel_T2 R) (rel_T2 R) (map_T2_pre id id id id f1 f2 id (rrename_T1 f1 f2) id (rrename_T2 f1 id) x2) y2 \<rbrakk>
+| "\<lbrakk> bij f1 ; |supp f1| <o |UNIV::'var set| ; id_on ((set7_T2_pre x2 \<union> \<Union>(FVars_T11 ` set9_T2_pre x2) \<union> \<Union>(FVars_T21 ` set11_T2_pre x2)) - set5_T2_pre x2) f1 ;
+     bij f2 ; |supp f2| <o |UNIV::'tyvar set| ; id_on (\<Union>(FVars_T12 ` set9_T2_pre x2) - set6_T2_pre x2) f2 ;
+    rel_T2_pre R (rel_T1 R) (rel_T1 R) (rel_T2 R) (rel_T2 R) (map_T2_pre id id id id f1 f2 f1 id (permute_T1 f1 f2) id (permute_T2 f1 id) x2) y2 \<rbrakk>
     \<Longrightarrow> rel_T2 R (T2_ctor x2) (T2_ctor y2)"
 
 (********************************)
@@ -158,17 +158,17 @@ lemma small_PFVars:
 lemma U1map_Uctor:
   fixes f1::"'var::{var_T1_pre, var_T2_pre} \<Rightarrow> 'var" and f2::"'tyvar::{var_T1_pre, var_T2_pre} \<Rightarrow> 'tyvar"
   assumes "bij f1" "|supp f1| <o |UNIV::'var set|" "bij f2" "|supp f2| <o |UNIV::'tyvar set|"
-  shows "validP p \<Longrightarrow> U1map f1 f2 (T1_ctor (map_T1_pre id id id id id id fst fst fst fst t)) (U1ctor y p) =
-    U1ctor (map_T1_pre f1 f2 id id f1 f2
-      (\<lambda>(t, pu). (rrename_T1 f1 f2 t, \<lambda>p. if validP p then U1map f1 f2 t (pu (Pmap (inv f1) (inv f2) p)) else undefined))
-      (\<lambda>(t, pu). (rrename_T1 f1 f2 t, \<lambda>p. if validP p then U1map f1 f2 t (pu (Pmap (inv f1) (inv f2) p)) else undefined))
-      (\<lambda>(t, pu). (rrename_T2 f1 f2 t, \<lambda>p. if validP p then U2map f1 f2 t (pu (Pmap (inv f1) (inv f2) p)) else undefined))
-      (\<lambda>(t, pu). (rrename_T2 f1 f2 t, \<lambda>p. if validP p then U2map f1 f2 t (pu (Pmap (inv f1) (inv f2) p)) else undefined))
+  shows "validP p \<Longrightarrow> U1map f1 f2 (T1_ctor (map_T1_pre id id id id id id id fst fst fst fst t)) (U1ctor y p) =
+    U1ctor (map_T1_pre f1 f2 id id f1 f2 f1
+      (\<lambda>(t, pu). (permute_T1 f1 f2 t, \<lambda>p. if validP p then U1map f1 f2 t (pu (Pmap (inv f1) (inv f2) p)) else undefined))
+      (\<lambda>(t, pu). (permute_T1 f1 f2 t, \<lambda>p. if validP p then U1map f1 f2 t (pu (Pmap (inv f1) (inv f2) p)) else undefined))
+      (\<lambda>(t, pu). (permute_T2 f1 f2 t, \<lambda>p. if validP p then U2map f1 f2 t (pu (Pmap (inv f1) (inv f2) p)) else undefined))
+      (\<lambda>(t, pu). (permute_T2 f1 f2 t, \<lambda>p. if validP p then U2map f1 f2 t (pu (Pmap (inv f1) (inv f2) p)) else undefined))
     y) (Pmap f1 f2 p)"
   apply (unfold U1ctor_def case_prod_beta fst_conv snd_conv)
   apply (erule conjE)+
   apply (rule trans)
-   apply (rule T1.rrename_cctors)
+   apply (rule permute_simps)
       apply (rule assms)+
   apply (subst T1_pre.map_comp)
               apply (rule bij_id supp_id_bound assms | assumption)+
@@ -231,17 +231,17 @@ lemma U1map_Uctor:
 lemma U2map_Uctor:
   fixes f1::"'var::{var_T1_pre, var_T2_pre} \<Rightarrow> 'var" and f2::"'tyvar::{var_T1_pre, var_T2_pre} \<Rightarrow> 'tyvar"
   assumes "bij f1" "|supp f1| <o |UNIV::'var set|" "bij f2" "|supp f2| <o |UNIV::'tyvar set|"
-  shows "validP p \<Longrightarrow> U2map f1 f2 (T2_ctor (map_T2_pre id id id id id id fst fst fst fst t)) (U2ctor y p) =
-    U2ctor (map_T2_pre f1 f2 id id f1 f2
-      (\<lambda>(t, pu). (rrename_T1 f1 f2 t, \<lambda>p. if validP p then U1map f1 f2 t (pu (Pmap (inv f1) (inv f2) p)) else undefined))
-      (\<lambda>(t, pu). (rrename_T1 f1 f2 t, \<lambda>p. if validP p then U1map f1 f2 t (pu (Pmap (inv f1) (inv f2) p)) else undefined))
-      (\<lambda>(t, pu). (rrename_T2 f1 f2 t, \<lambda>p. if validP p then U2map f1 f2 t (pu (Pmap (inv f1) (inv f2) p)) else undefined))
-      (\<lambda>(t, pu). (rrename_T2 f1 f2 t, \<lambda>p. if validP p then U2map f1 f2 t (pu (Pmap (inv f1) (inv f2) p)) else undefined))
+  shows "validP p \<Longrightarrow> U2map f1 f2 (T2_ctor (map_T2_pre id id id id id id id fst fst fst fst t)) (U2ctor y p) =
+    U2ctor (map_T2_pre f1 f2 id id f1 f2 f1
+      (\<lambda>(t, pu). (permute_T1 f1 f2 t, \<lambda>p. if validP p then U1map f1 f2 t (pu (Pmap (inv f1) (inv f2) p)) else undefined))
+      (\<lambda>(t, pu). (permute_T1 f1 f2 t, \<lambda>p. if validP p then U1map f1 f2 t (pu (Pmap (inv f1) (inv f2) p)) else undefined))
+      (\<lambda>(t, pu). (permute_T2 f1 f2 t, \<lambda>p. if validP p then U2map f1 f2 t (pu (Pmap (inv f1) (inv f2) p)) else undefined))
+      (\<lambda>(t, pu). (permute_T2 f1 f2 t, \<lambda>p. if validP p then U2map f1 f2 t (pu (Pmap (inv f1) (inv f2) p)) else undefined))
     y) (Pmap f1 f2 p)"
   apply (unfold U2ctor_def case_prod_beta fst_conv snd_conv)
   apply (erule conjE)+
   apply (rule trans)
-   apply (rule T1.rrename_cctors)
+   apply (rule permute_simps)
       apply (rule assms)+
   apply (subst T2_pre.map_comp)
               apply (rule bij_id supp_id_bound assms | assumption)+
@@ -303,22 +303,35 @@ lemma U2map_Uctor:
   done
 
 lemma U1FVars_subsets:
-  "validP p \<Longrightarrow> set5_T1_pre (y::(_, _, 'a::{var_T1_pre,var_T2_pre}, 'b, _, _, _, _, _, _) T1_pre) \<inter> (PFVars_1 p \<union> {}) = {} \<Longrightarrow>
-  (\<And>t pu p. validP p \<Longrightarrow> (t, pu) \<in> set7_T1_pre y \<union> set8_T1_pre y \<Longrightarrow> U1FVars_1 t (pu p) \<subseteq> FFVars_T11 t \<union> PFVars_1 p \<union> {}) \<Longrightarrow>
-  (\<And>t pu p. validP p \<Longrightarrow> (t, pu) \<in> set9_T1_pre y \<union> set10_T1_pre y \<Longrightarrow> U2FVars_1 t (pu p) \<subseteq> FFVars_T21 t \<union> PFVars_1 p \<union> {}) \<Longrightarrow>
-  U1FVars_1 (T1_ctor (map_T1_pre id id id id id id fst fst fst fst y)) (U1ctor y p) \<subseteq> FFVars_T11 (T1_ctor (map_T1_pre id id id id id id fst fst fst fst y)) \<union> PFVars_1 p \<union> {}"
-  "validP p \<Longrightarrow> set6_T1_pre (y::(_, _, 'a::{var_T1_pre,var_T2_pre}, 'b, _, _, _, _, _, _) T1_pre) \<inter> (PFVars_2 p \<union> {}) = {} \<Longrightarrow>
-  (\<And>t pu p. validP p \<Longrightarrow> (t, pu) \<in> set7_T1_pre y \<union> set8_T1_pre y \<Longrightarrow> U1FVars_2 t (pu p) \<subseteq> FFVars_T12 t \<union> PFVars_2 p \<union> {}) \<Longrightarrow>
-  (\<And>t pu p. validP p \<Longrightarrow> (t, pu) \<in> set9_T1_pre y \<union> set10_T1_pre y \<Longrightarrow> U2FVars_2 t (pu p) \<subseteq> FFVars_T22 t \<union> PFVars_2 p \<union> {}) \<Longrightarrow>
-  U1FVars_2 (T1_ctor (map_T1_pre id id id id id id fst fst fst fst y)) (U1ctor y p) \<subseteq> FFVars_T12 (T1_ctor (map_T1_pre id id id id id id fst fst fst fst y)) \<union> PFVars_2 p \<union> {}"
-   apply (unfold case_prod_beta U1ctor_def Un_empty_right T1.FFVars_cctors)
+  "validP p \<Longrightarrow> set5_T1_pre (y::(_, _, 'a::{var_T1_pre,var_T2_pre}, 'b, _, _, _, _, _, _, _) T1_pre) \<inter> (PFVars_1 p \<union> {}) = {} \<Longrightarrow>
+  (\<And>t pu p. validP p \<Longrightarrow> (t, pu) \<in> set8_T1_pre y \<union> set9_T1_pre y \<Longrightarrow> U1FVars_1 t (pu p) \<subseteq> FVars_T11 t \<union> PFVars_1 p \<union> {}) \<Longrightarrow>
+  (\<And>t pu p. validP p \<Longrightarrow> (t, pu) \<in> set10_T1_pre y \<union> set11_T1_pre y \<Longrightarrow> U2FVars_1 t (pu p) \<subseteq> FVars_T21 t \<union> PFVars_1 p \<union> {}) \<Longrightarrow>
+  U1FVars_1 (T1_ctor (map_T1_pre id id id id id id id fst fst fst fst y)) (U1ctor y p) \<subseteq> FVars_T11 (T1_ctor (map_T1_pre id id id id id id id fst fst fst fst y)) \<union> PFVars_1 p \<union> {}"
+  "validP p \<Longrightarrow> set6_T1_pre (y::(_, _, 'a::{var_T1_pre,var_T2_pre}, 'b, _, _, _, _, _, _, _) T1_pre) \<inter> (PFVars_2 p \<union> {}) = {} \<Longrightarrow>
+  (\<And>t pu p. validP p \<Longrightarrow> (t, pu) \<in> set8_T1_pre y \<union> set9_T1_pre y \<Longrightarrow> U1FVars_2 t (pu p) \<subseteq> FVars_T12 t \<union> PFVars_2 p \<union> {}) \<Longrightarrow>
+  (\<And>t pu p. validP p \<Longrightarrow> (t, pu) \<in> set10_T1_pre y \<union> set11_T1_pre y \<Longrightarrow> U2FVars_2 t (pu p) \<subseteq> FVars_T22 t \<union> PFVars_2 p \<union> {}) \<Longrightarrow>
+  U1FVars_2 (T1_ctor (map_T1_pre id id id id id id id fst fst fst fst y)) (U1ctor y p) \<subseteq> FVars_T12 (T1_ctor (map_T1_pre id id id id id id id fst fst fst fst y)) \<union> PFVars_2 p \<union> {}"
+   apply (unfold case_prod_beta U1ctor_def Un_empty_right FVars_ctors)
   apply (erule conjE)+
   subgoal premises prems
     apply (subst T1_pre.set_map, (rule bij_id supp_id_bound prems)+)+
     apply (unfold image_id image_comp comp_def)
     apply (rule Un_mono')+
       (* REPEAT_DETERM FIRST' *)
-        apply (rule iffD1[OF arg_cong2[OF refl Un_commute, of "(\<subseteq>)"] image_imsupp_subset])
+      (* TRY
+          apply (rule iffD2[OF arg_cong2[OF refl, of _ _ "(\<subseteq>)"]])
+          apply (rule Diff_Un_disjunct)
+          apply (rule prems)
+          apply (rule Diff_mono[OF _ subset_refl])
+       *)
+       apply (rule iffD1[OF arg_cong2[OF refl Un_commute, of "(\<subseteq>)"] image_imsupp_subset])
+      (* repeated *)
+      (* TRY *)
+        apply (rule iffD2[OF arg_cong2[OF refl, of _ _ "(\<subseteq>)"]])
+        apply (rule Diff_Un_disjunct)
+        apply (rule prems)
+        apply (rule Diff_mono[OF _ subset_refl])
+       apply (rule iffD1[OF arg_cong2[OF refl Un_commute, of "(\<subseteq>)"] image_imsupp_subset])
       (* orelse *)
       (* TRY
           apply (rule iffD2[OF arg_cong2[OF refl, of _ _ "(\<subseteq>)"]])
@@ -467,21 +480,34 @@ lemma U1FVars_subsets:
   done
 
 lemma U2FVars_subsets:
-  "validP p \<Longrightarrow> set5_T2_pre (y::(_, _, 'a::{var_T1_pre,var_T2_pre}, 'b, _, _, _, _, _, _) T2_pre) \<inter> (PFVars_1 p \<union> {}) = {} \<Longrightarrow>
-  (\<And>t pu p. validP p \<Longrightarrow> (t, pu) \<in> set7_T2_pre y \<union> set8_T2_pre y \<Longrightarrow> U1FVars_1 t (pu p) \<subseteq> FFVars_T11 t \<union> PFVars_1 p \<union> {}) \<Longrightarrow>
-  (\<And>t pu p. validP p \<Longrightarrow> (t, pu) \<in> set9_T2_pre y \<union> set10_T2_pre y \<Longrightarrow> U2FVars_1 t (pu p) \<subseteq> FFVars_T21 t \<union> PFVars_1 p \<union> {}) \<Longrightarrow>
-  U2FVars_1 (T2_ctor (map_T2_pre id id id id id id fst fst fst fst y)) (U2ctor y p) \<subseteq> FFVars_T21 (T2_ctor (map_T2_pre id id id id id id fst fst fst fst y)) \<union> PFVars_1 p \<union> {}"
-  "validP p \<Longrightarrow> set6_T2_pre (y::(_, _, 'a::{var_T1_pre,var_T2_pre}, 'b, _, _, _, _, _, _) T2_pre) \<inter> (PFVars_2 p \<union> {}) = {} \<Longrightarrow>
-  (\<And>t pu p. validP p \<Longrightarrow> (t, pu) \<in> set7_T2_pre y \<union> set8_T2_pre y \<Longrightarrow> U1FVars_2 t (pu p) \<subseteq> FFVars_T12 t \<union> PFVars_2 p \<union> {}) \<Longrightarrow>
-  (\<And>t pu p. validP p \<Longrightarrow> (t, pu) \<in> set9_T2_pre y \<union> set10_T2_pre y \<Longrightarrow> U2FVars_2 t (pu p) \<subseteq> FFVars_T22 t \<union> PFVars_2 p \<union> {}) \<Longrightarrow>
-  U2FVars_2 (T2_ctor (map_T2_pre id id id id id id fst fst fst fst y)) (U2ctor y p) \<subseteq> FFVars_T22 (T2_ctor (map_T2_pre id id id id id id fst fst fst fst y)) \<union> PFVars_2 p \<union> {}"
-   apply (unfold case_prod_beta U2ctor_def Un_empty_right T1.FFVars_cctors)
+  "validP p \<Longrightarrow> set5_T2_pre (y::(_, _, 'a::{var_T1_pre,var_T2_pre}, 'b, _, _, _, _, _, _, _) T2_pre) \<inter> (PFVars_1 p \<union> {}) = {} \<Longrightarrow>
+  (\<And>t pu p. validP p \<Longrightarrow> (t, pu) \<in> set8_T2_pre y \<union> set9_T2_pre y \<Longrightarrow> U1FVars_1 t (pu p) \<subseteq> FVars_T11 t \<union> PFVars_1 p \<union> {}) \<Longrightarrow>
+  (\<And>t pu p. validP p \<Longrightarrow> (t, pu) \<in> set10_T2_pre y \<union> set11_T2_pre y \<Longrightarrow> U2FVars_1 t (pu p) \<subseteq> FVars_T21 t \<union> PFVars_1 p \<union> {}) \<Longrightarrow>
+  U2FVars_1 (T2_ctor (map_T2_pre id id id id id id id fst fst fst fst y)) (U2ctor y p) \<subseteq> FVars_T21 (T2_ctor (map_T2_pre id id id id id id id fst fst fst fst y)) \<union> PFVars_1 p \<union> {}"
+  "validP p \<Longrightarrow> set6_T2_pre (y::(_, _, 'a::{var_T1_pre,var_T2_pre}, 'b, _, _, _, _, _, _, _) T2_pre) \<inter> (PFVars_2 p \<union> {}) = {} \<Longrightarrow>
+  (\<And>t pu p. validP p \<Longrightarrow> (t, pu) \<in> set8_T2_pre y \<union> set9_T2_pre y \<Longrightarrow> U1FVars_2 t (pu p) \<subseteq> FVars_T12 t \<union> PFVars_2 p \<union> {}) \<Longrightarrow>
+  (\<And>t pu p. validP p \<Longrightarrow> (t, pu) \<in> set10_T2_pre y \<union> set11_T2_pre y \<Longrightarrow> U2FVars_2 t (pu p) \<subseteq> FVars_T22 t \<union> PFVars_2 p \<union> {}) \<Longrightarrow>
+  U2FVars_2 (T2_ctor (map_T2_pre id id id id id id id fst fst fst fst y)) (U2ctor y p) \<subseteq> FVars_T22 (T2_ctor (map_T2_pre id id id id id id id fst fst fst fst y)) \<union> PFVars_2 p \<union> {}"
+   apply (unfold case_prod_beta U2ctor_def Un_empty_right FVars_ctors)
   apply (erule conjE)+
   subgoal premises prems
     apply (subst T2_pre.set_map, (rule bij_id supp_id_bound prems)+)+
     apply (unfold image_id image_comp comp_def)
     apply (rule Un_mono')+
       (* REPEAT_DETERM FIRST' *)
+      (* TRY
+          apply (rule iffD2[OF arg_cong2[OF refl, of _ _ "(\<subseteq>)"]])
+          apply (rule Diff_Un_disjunct)
+          apply (rule prems)
+          apply (rule Diff_mono[OF _ subset_refl])
+        *)
+        apply (rule iffD1[OF arg_cong2[OF refl Un_commute, of "(\<subseteq>)"] image_imsupp_subset])
+      (* repeated *)
+      (* TRY *)
+        apply (rule iffD2[OF arg_cong2[OF refl, of _ _ "(\<subseteq>)"]])
+        apply (rule Diff_Un_disjunct)
+        apply (rule prems)
+        apply (rule Diff_mono[OF _ subset_refl])
         apply (rule iffD1[OF arg_cong2[OF refl Un_commute, of "(\<subseteq>)"] image_imsupp_subset])
       (* orelse *)
       (* TRY
@@ -691,11 +717,11 @@ val T1_model = {
   axioms = {
     Umap_id0 = fn ctxt => EVERY1 [
       resolve_tac ctxt [trans],
-      resolve_tac ctxt @{thms T1.rrename_id0s[THEN fun_cong]},
+      resolve_tac ctxt @{thms permute_id0s[THEN fun_cong]},
       resolve_tac ctxt @{thms id_apply}
     ],
-    Umap_comp0 = fn ctxt => resolve_tac ctxt @{thms T1.rrename_comp0s[symmetric, THEN fun_cong]} 1 THEN REPEAT_DETERM (assume_tac ctxt 1),
-    Umap_cong_id = fn ctxt => resolve_tac ctxt @{thms T1.rrename_cong_ids} 1 THEN REPEAT_DETERM (assume_tac ctxt 1 ORELSE Goal.assume_rule_tac ctxt 1),
+    Umap_comp0 = fn ctxt => resolve_tac ctxt @{thms permute_comp0s[symmetric, THEN fun_cong]} 1 THEN REPEAT_DETERM (assume_tac ctxt 1),
+    Umap_cong_id = fn ctxt => resolve_tac ctxt @{thms permute_cong_ids} 1 THEN REPEAT_DETERM (assume_tac ctxt 1 ORELSE Goal.assume_rule_tac ctxt 1),
     Umap_Uctor = fn ctxt => EVERY1 [
       K (Local_Defs.unfold0_tac ctxt @{thms if_True}),
       resolve_tac ctxt @{thms U1map_Uctor},
@@ -725,17 +751,24 @@ val T2_model = {
   axioms = {
     Umap_id0 = fn ctxt => EVERY1 [
       resolve_tac ctxt [trans],
-      resolve_tac ctxt @{thms T1.rrename_id0s[THEN fun_cong]},
+      resolve_tac ctxt @{thms permute_id0s[THEN fun_cong]},
       resolve_tac ctxt @{thms id_apply}
     ],
-    Umap_comp0 = fn ctxt => resolve_tac ctxt @{thms T1.rrename_comp0s[symmetric, THEN fun_cong]} 1 THEN REPEAT_DETERM (assume_tac ctxt 1),
-    Umap_cong_id = fn ctxt => resolve_tac ctxt @{thms T1.rrename_cong_ids} 1 THEN REPEAT_DETERM (assume_tac ctxt 1 ORELSE Goal.assume_rule_tac ctxt 1),
+    Umap_comp0 = fn ctxt => resolve_tac ctxt @{thms permute_comp0s[symmetric, THEN fun_cong]} 1 THEN REPEAT_DETERM (assume_tac ctxt 1),
+    Umap_cong_id = fn ctxt => resolve_tac ctxt @{thms permute_cong_ids} 1 THEN REPEAT_DETERM (assume_tac ctxt 1 ORELSE Goal.assume_rule_tac ctxt 1),
     Umap_Uctor = fn ctxt => resolve_tac ctxt @{thms U2map_Uctor} 1 THEN REPEAT_DETERM (assume_tac ctxt 1),
     UFVars_subsets = replicate nvars (fn ctxt => resolve_tac ctxt @{thms U2FVars_subsets} 1 THEN REPEAT_DETERM (assume_tac ctxt 1 ORELSE Goal.assume_rule_tac ctxt 1))
   }
 };
 
-val fp_res = the (MRBNF_FP_Def_Sugar.fp_result_of @{context} "Fixpoint.T1")
+val fp_res = the (MRBNF_FP_Def_Sugar.fp_result_of @{context} "Least_Fixpoint.T1")
+\<close>
+
+ML_file \<open>../Tools/mrbnf_recursor_tactics.ML\<close>
+ML_file \<open>../Tools/mrbnf_recursor.ML\<close>
+
+ML \<open>
+Multithreading.parallel_proofs := 0
 \<close>
 
 local_setup \<open>fn lthy =>
@@ -1504,10 +1537,10 @@ lemma vvsubst_rrenames:
   fixes f1::"'var::{var_T1_pre,var_T2_pre} \<Rightarrow> 'var" and f2::"'tyvar::{var_T1_pre,var_T2_pre} \<Rightarrow> 'tyvar"
   assumes f_prems: "bij f1" "|supp f1| <o |UNIV::'var set|" "bij f2" "|supp f2| <o |UNIV::'tyvar set|"
   shows
-    "vvsubst_T1 f1 f2 (id::'a::{var_T1_pre,var_T2_pre} \<Rightarrow> 'a) (id::'b \<Rightarrow> 'b) = rrename_T1 f1 f2"
-    "vvsubst_T2 f1 f2 (id::'a::{var_T1_pre,var_T2_pre} \<Rightarrow> 'a) (id::'b \<Rightarrow> 'b) = rrename_T2 f1 f2"
+    "vvsubst_T1 f1 f2 (id::'a::{var_T1_pre,var_T2_pre} \<Rightarrow> 'a) (id::'b \<Rightarrow> 'b) = permute_T1 f1 f2"
+    "vvsubst_T2 f1 f2 (id::'a::{var_T1_pre,var_T2_pre} \<Rightarrow> 'a) (id::'b \<Rightarrow> 'b) = permute_T2 f1 f2"
 proof -
-  have x: "\<And>(x::('var, 'tyvar, 'a, 'b) T1) (y::('var, 'tyvar, 'a, 'b) T2). vvsubst_T1 f1 f2 id id x = rrename_T1 f1 f2 x \<and> vvsubst_T2 f1 f2 id id y = rrename_T2 f1 f2 y"
+  have x: "\<And>(x::('var, 'tyvar, 'a, 'b) T1) (y::('var, 'tyvar, 'a, 'b) T2). vvsubst_T1 f1 f2 id id x = permute_T1 f1 f2 x \<and> vvsubst_T2 f1 f2 id id y = permute_T2 f1 f2 y"
     subgoal for x y
       apply (rule T1.TT_fresh_co_induct[of _ _ _ _ x y])
         (* REPEAT_DETERM *)
@@ -1542,7 +1575,7 @@ proof -
         apply assumption
        apply (rule sym)
        apply (rule trans)
-        apply (rule T1.rrename_cctors)
+        apply (rule T1.permute_cctors)
            apply (rule f_prems)+
       apply (rule arg_cong[OF T1_pre.map_cong])
                           apply (rule f_prems supp_id_bound bij_id refl)+
@@ -1589,7 +1622,7 @@ proof -
        apply assumption
       apply (rule sym)
       apply (rule trans)
-       apply (rule T1.rrename_cctors)
+       apply (rule T1.permute_cctors)
           apply (rule f_prems)+
       apply (rule arg_cong[of _ _ T2_ctor])
       apply (rule T2_pre.map_cong)
@@ -1618,12 +1651,12 @@ proof -
          apply (rule sym, assumption)+
       done
     done
-  show "vvsubst_T1 f1 f2 (id::'a::{var_T1_pre,var_T2_pre} \<Rightarrow> 'a) (id::'b \<Rightarrow> 'b) = rrename_T1 f1 f2"
+  show "vvsubst_T1 f1 f2 (id::'a::{var_T1_pre,var_T2_pre} \<Rightarrow> 'a) (id::'b \<Rightarrow> 'b) = permute_T1 f1 f2"
     apply (rule ext)
     apply (rule conjunct1[OF x])
     done
 
-  show "vvsubst_T2 f1 f2 (id::'a::{var_T1_pre,var_T2_pre} \<Rightarrow> 'a) (id::'b \<Rightarrow> 'b) = rrename_T2 f1 f2"
+  show "vvsubst_T2 f1 f2 (id::'a::{var_T1_pre,var_T2_pre} \<Rightarrow> 'a) (id::'b \<Rightarrow> 'b) = permute_T2 f1 f2"
     apply (rule ext)
     apply (rule conjunct2[OF x])
     done
@@ -1673,28 +1706,28 @@ lemma rel_imp_rrename:
     and x::"('var, 'tyvar, 'a::{var_T1_pre,var_T2_pre}, 'b) T1"
     and x2::"('var, 'tyvar, 'a, 'b) T2"
   assumes "bij f1" "|supp f1| <o |UNIV::'var set|" "bij f2" "|supp f2| <o |UNIV::'tyvar set|"
-  shows "rel_T1 R (rrename_T1 f1 f2 x) (rrename_T1 f1 f2 y) \<Longrightarrow> rel_T1 R x y"
-    "rel_T2 R (rrename_T2 f1 f2 x2) (rrename_T2 f1 f2 y2) \<Longrightarrow> rel_T2 R x2 y2"
+  shows "rel_T1 R (permute_T1 f1 f2 x) (permute_T1 f1 f2 y) \<Longrightarrow> rel_T1 R x y"
+    "rel_T2 R (permute_T2 f1 f2 x2) (permute_T2 f1 f2 y2) \<Longrightarrow> rel_T2 R x2 y2"
 proof -
-  have x: "(\<forall>(R::'b \<Rightarrow> 'c \<Rightarrow> bool) (x::('var, 'tyvar, 'a, 'b) T1) y. rel_T1 R (rrename_T1 f1 f2 x) (rrename_T1 f1 f2 y) \<longrightarrow> rel_T1 R x y)
-    \<and> (\<forall>(R::'b \<Rightarrow> 'c \<Rightarrow> bool) (x::('var, 'tyvar, 'a, 'b) T2) y. rel_T2 R (rrename_T2 f1 f2 x) (rrename_T2 f1 f2 y) \<longrightarrow> rel_T2 R x y)"
+  have x: "(\<forall>(R::'b \<Rightarrow> 'c \<Rightarrow> bool) (x::('var, 'tyvar, 'a, 'b) T1) y. rel_T1 R (permute_T1 f1 f2 x) (permute_T1 f1 f2 y) \<longrightarrow> rel_T1 R x y)
+    \<and> (\<forall>(R::'b \<Rightarrow> 'c \<Rightarrow> bool) (x::('var, 'tyvar, 'a, 'b) T2) y. rel_T2 R (permute_T2 f1 f2 x) (permute_T2 f1 f2 y) \<longrightarrow> rel_T2 R x y)"
     apply (rule rel_T1_rel_T2.coinduct)
      apply (erule rel_plain_cases)
       (* REPEAT twice *)
-     apply (drule arg_cong[of _ _ "rrename_T1 (inv f1) (inv f2)"])
-     apply (subst (asm) T1.rrename_comps inv_o_simp1, (rule assms bij_imp_bij_inv supp_inv_bound)+)+
-     apply (unfold T1.rrename_ids)
+     apply (drule arg_cong[of _ _ "permute_T1 (inv f1) (inv f2)"])
+     apply (subst (asm) T1.permute_comps inv_o_simp1, (rule assms bij_imp_bij_inv supp_inv_bound)+)+
+     apply (unfold T1.permute_ids)
       (* repeated *)
-     apply (drule arg_cong[of _ _ "rrename_T1 (inv f1) (inv f2)"])
-     apply (subst (asm) T1.rrename_comps inv_o_simp1, (rule assms bij_imp_bij_inv supp_inv_bound)+)+
-     apply (unfold T1.rrename_ids)
+     apply (drule arg_cong[of _ _ "permute_T1 (inv f1) (inv f2)"])
+     apply (subst (asm) T1.permute_comps inv_o_simp1, (rule assms bij_imp_bij_inv supp_inv_bound)+)+
+     apply (unfold T1.permute_ids)
       (* END REPEAT twice *)
      apply hypsubst
      apply (rule exI)+
      apply (rule conjI, rule refl)+
-     apply (rule conjI, rule T1.rrename_cctors, (rule assms bij_imp_bij_inv supp_inv_bound)+)+
+     apply (rule conjI, rule T1.permute_cctors, (rule assms bij_imp_bij_inv supp_inv_bound)+)+
      apply (rule conjI bij_id supp_id_bound id_on_id)+
-     apply (unfold T1.rrename_id0s T1_pre.map_id T1_pre.mr_rel_id)
+     apply (unfold T1.permute_id0s T1_pre.map_id T1_pre.mr_rel_id)
      apply (rule iffD2[OF T1_pre.mr_rel_map(1)])
                    apply (rule supp_inv_bound assms supp_id_bound bij_imp_bij_inv bij_id)+
      apply (unfold id_o o_id Grp_UNIV_id eq_OO)
@@ -1709,8 +1742,8 @@ proof -
                       apply (unfold Grp_UNIV_def)[1]
                       apply hypsubst
                       apply (rule disjI1)
-                      apply (subst T1.rrename_comps inv_o_simp2, (rule bij_imp_bij_inv assms supp_inv_bound)+)+
-                      apply (unfold T1.rrename_ids)
+                      apply (subst T1.permute_comps inv_o_simp2, (rule bij_imp_bij_inv assms supp_inv_bound)+)+
+                      apply (unfold T1.permute_ids)
                       apply assumption
       (* repeated *)
                      apply (rule ballI impI)+
@@ -1719,8 +1752,8 @@ proof -
                      apply (unfold Grp_UNIV_def)[1]
                      apply hypsubst
                      apply (rule disjI1)
-                     apply (subst T1.rrename_comps inv_o_simp2, (rule bij_imp_bij_inv assms supp_inv_bound)+)+
-                     apply (unfold T1.rrename_ids)
+                     apply (subst T1.permute_comps inv_o_simp2, (rule bij_imp_bij_inv assms supp_inv_bound)+)+
+                     apply (unfold T1.permute_ids)
                      apply assumption
       (* repeated *)
                     apply (rule ballI impI)+
@@ -1729,8 +1762,8 @@ proof -
                     apply (unfold Grp_UNIV_def)[1]
                     apply hypsubst
                     apply (rule disjI1)
-                    apply (subst T1.rrename_comps inv_o_simp2, (rule bij_imp_bij_inv assms supp_inv_bound)+)+
-                    apply (unfold T1.rrename_ids)
+                    apply (subst T1.permute_comps inv_o_simp2, (rule bij_imp_bij_inv assms supp_inv_bound)+)+
+                    apply (unfold T1.permute_ids)
                     apply assumption
       (* repeated *)
                    apply (rule ballI impI)+
@@ -1739,28 +1772,28 @@ proof -
                    apply (unfold Grp_UNIV_def)[1]
                    apply hypsubst
                    apply (rule disjI1)
-                   apply (subst T1.rrename_comps inv_o_simp2, (rule bij_imp_bij_inv assms supp_inv_bound)+)+
-                   apply (unfold T1.rrename_ids)
+                   apply (subst T1.permute_comps inv_o_simp2, (rule bij_imp_bij_inv assms supp_inv_bound)+)+
+                   apply (unfold T1.permute_ids)
                    apply assumption
       (* END REPEAT_DETERM *)
                   apply (rule supp_inv_bound assms supp_id_bound bij_imp_bij_inv)+
       (* second type, same tactic *)
     apply (erule rel_plain_cases)
       (* REPEAT twice *)
-    apply (drule arg_cong[of _ _ "rrename_T2 (inv f1) (inv f2)"])
-    apply (subst (asm) T1.rrename_comps inv_o_simp1, (rule assms bij_imp_bij_inv supp_inv_bound)+)+
-    apply (unfold T1.rrename_ids)
+    apply (drule arg_cong[of _ _ "permute_T2 (inv f1) (inv f2)"])
+    apply (subst (asm) T1.permute_comps inv_o_simp1, (rule assms bij_imp_bij_inv supp_inv_bound)+)+
+    apply (unfold T1.permute_ids)
       (* repeated *)
-    apply (drule arg_cong[of _ _ "rrename_T2 (inv f1) (inv f2)"])
-    apply (subst (asm) T1.rrename_comps inv_o_simp1, (rule assms bij_imp_bij_inv supp_inv_bound)+)+
-    apply (unfold T1.rrename_ids)
+    apply (drule arg_cong[of _ _ "permute_T2 (inv f1) (inv f2)"])
+    apply (subst (asm) T1.permute_comps inv_o_simp1, (rule assms bij_imp_bij_inv supp_inv_bound)+)+
+    apply (unfold T1.permute_ids)
       (* END REPEAT twice *)
     apply hypsubst
     apply (rule exI)+
     apply (rule conjI, rule refl)+
-    apply (rule conjI, rule T1.rrename_cctors, (rule assms bij_imp_bij_inv supp_inv_bound)+)+
+    apply (rule conjI, rule T1.permute_cctors, (rule assms bij_imp_bij_inv supp_inv_bound)+)+
     apply (rule conjI bij_id supp_id_bound id_on_id)+
-    apply (unfold T1.rrename_id0s T2_pre.map_id T2_pre.mr_rel_id)
+    apply (unfold T1.permute_id0s T2_pre.map_id T2_pre.mr_rel_id)
     apply (rule iffD2[OF T2_pre.mr_rel_map(1)])
                   apply (rule supp_inv_bound assms supp_id_bound bij_imp_bij_inv bij_id)+
     apply (unfold id_o o_id Grp_UNIV_id eq_OO)
@@ -1775,8 +1808,8 @@ proof -
                      apply (unfold Grp_UNIV_def)[1]
                      apply hypsubst
                      apply (rule disjI1)
-                     apply (subst T1.rrename_comps inv_o_simp2, (rule bij_imp_bij_inv assms supp_inv_bound)+)+
-                     apply (unfold T1.rrename_ids)
+                     apply (subst T1.permute_comps inv_o_simp2, (rule bij_imp_bij_inv assms supp_inv_bound)+)+
+                     apply (unfold T1.permute_ids)
                      apply assumption
       (* repeated *)
                     apply (rule ballI impI)+
@@ -1785,8 +1818,8 @@ proof -
                     apply (unfold Grp_UNIV_def)[1]
                     apply hypsubst
                     apply (rule disjI1)
-                    apply (subst T1.rrename_comps inv_o_simp2, (rule bij_imp_bij_inv assms supp_inv_bound)+)+
-                    apply (unfold T1.rrename_ids)
+                    apply (subst T1.permute_comps inv_o_simp2, (rule bij_imp_bij_inv assms supp_inv_bound)+)+
+                    apply (unfold T1.permute_ids)
                     apply assumption
       (* repeated *)
                    apply (rule ballI impI)+
@@ -1795,8 +1828,8 @@ proof -
                    apply (unfold Grp_UNIV_def)[1]
                    apply hypsubst
                    apply (rule disjI1)
-                   apply (subst T1.rrename_comps inv_o_simp2, (rule bij_imp_bij_inv assms supp_inv_bound)+)+
-                   apply (unfold T1.rrename_ids)
+                   apply (subst T1.permute_comps inv_o_simp2, (rule bij_imp_bij_inv assms supp_inv_bound)+)+
+                   apply (unfold T1.permute_ids)
                    apply assumption
       (* repeated *)
                   apply (rule ballI impI)+
@@ -1805,20 +1838,20 @@ proof -
                   apply (unfold Grp_UNIV_def)[1]
                   apply hypsubst
                   apply (rule disjI1)
-                  apply (subst T1.rrename_comps inv_o_simp2, (rule bij_imp_bij_inv assms supp_inv_bound)+)+
-                  apply (unfold T1.rrename_ids)
+                  apply (subst T1.permute_comps inv_o_simp2, (rule bij_imp_bij_inv assms supp_inv_bound)+)+
+                  apply (unfold T1.permute_ids)
                   apply assumption
       (* END REPEAT_DETERM *)
                  apply (rule supp_inv_bound assms supp_id_bound bij_imp_bij_inv)+
     done
 
-  show "rel_T1 R (rrename_T1 f1 f2 x) (rrename_T1 f1 f2 y) \<Longrightarrow> rel_T1 R x y"
+  show "rel_T1 R (permute_T1 f1 f2 x) (permute_T1 f1 f2 y) \<Longrightarrow> rel_T1 R x y"
     apply (erule mp[rotated])
     apply (insert x)
     apply (erule conjE allE)+
     apply assumption
     done
-  show "rel_T2 R (rrename_T2 f1 f2 x2) (rrename_T2 f1 f2 y2) \<Longrightarrow> rel_T2 R x2 y2"
+  show "rel_T2 R (permute_T2 f1 f2 x2) (permute_T2 f1 f2 y2) \<Longrightarrow> rel_T2 R x2 y2"
     apply (erule mp[rotated])
     apply (insert x)
     apply (erule conjE allE)+
@@ -1831,17 +1864,17 @@ lemma rel_rrename:
     and x::"('var, 'tyvar, 'a::{var_T1_pre,var_T2_pre}, 'b) T1"
     and x2::"('var, 'tyvar, 'a, 'b) T2"
   assumes "bij f1" "|supp f1| <o |UNIV::'var set|" "bij f2" "|supp f2| <o |UNIV::'tyvar set|"
-  shows "rel_T1 R (rrename_T1 f1 f2 x) (rrename_T1 f1 f2 y) = rel_T1 R x y"
-    "rel_T2 R (rrename_T2 f1 f2 x2) (rrename_T2 f1 f2 y2) = rel_T2 R x2 y2"
+  shows "rel_T1 R (permute_T1 f1 f2 x) (permute_T1 f1 f2 y) = rel_T1 R x y"
+    "rel_T2 R (permute_T2 f1 f2 x2) (permute_T2 f1 f2 y2) = rel_T2 R x2 y2"
   subgoal
     apply (rule iffI)
      apply (erule rel_imp_rrename[rotated -1])
         apply (rule assms)+
     apply (rule rel_imp_rrename[rotated -1])
-        apply (subst T1.rrename_comps)
+        apply (subst T1.permute_comps)
                 prefer 9 (* 4 * nvars + 1 *)
-                apply (subst inv_o_simp1 T1.rrename_comps, (rule assms bij_imp_bij_inv supp_inv_bound)+)+
-                apply (unfold T1.rrename_ids)
+                apply (subst inv_o_simp1 T1.permute_comps, (rule assms bij_imp_bij_inv supp_inv_bound)+)+
+                apply (unfold T1.permute_ids)
                 apply assumption
                apply (rule assms bij_imp_bij_inv supp_inv_bound)+
     done
@@ -1850,10 +1883,10 @@ lemma rel_rrename:
      apply (erule rel_imp_rrename[rotated -1])
         apply (rule assms)+
     apply (rule rel_imp_rrename[rotated -1])
-        apply (subst T1.rrename_comps)
+        apply (subst T1.permute_comps)
                 prefer 9 (* 4 * nvars + 1 *)
-                apply (subst inv_o_simp1 T1.rrename_comps, (rule assms bij_imp_bij_inv supp_inv_bound)+)+
-                apply (unfold T1.rrename_ids)
+                apply (subst inv_o_simp1 T1.permute_comps, (rule assms bij_imp_bij_inv supp_inv_bound)+)+
+                apply (unfold T1.permute_ids)
                 apply assumption
                apply (rule assms bij_imp_bij_inv supp_inv_bound)+
     done
@@ -1864,26 +1897,26 @@ lemma rel_FFVars:
     and x::"('var::{var_T1_pre,var_T2_pre}, 'tyvar::{var_T1_pre,var_T2_pre}, 'a::{var_T1_pre,var_T2_pre}, 'b) T1"
     and x2::"('var, 'tyvar, 'a, 'b) T2"
   shows
-    "rel_T1 R x y \<Longrightarrow> FFVars_T11 x = FFVars_T11 y"
-    "rel_T1 R x y \<Longrightarrow> FFVars_T12 x = FFVars_T12 y"
-    "rel_T2 R x2 y2 \<Longrightarrow> FFVars_T21 x2 = FFVars_T21 y2"
-    "rel_T2 R x2 y2 \<Longrightarrow> FFVars_T22 x2 = FFVars_T22 y2"
+    "rel_T1 R x y \<Longrightarrow> FVars_T11 x = FVars_T11 y"
+    "rel_T1 R x y \<Longrightarrow> FVars_T12 x = FVars_T12 y"
+    "rel_T2 R x2 y2 \<Longrightarrow> FVars_T21 x2 = FVars_T21 y2"
+    "rel_T2 R x2 y2 \<Longrightarrow> FVars_T22 x2 = FVars_T22 y2"
 proof -
   have x: "(\<forall>y f1 f2. bij f1 \<longrightarrow> |supp f1| <o |UNIV::'var set| \<longrightarrow> bij f2 \<longrightarrow> |supp f2| <o |UNIV::'tyvar set|
-    \<longrightarrow> rel_T1 R (rrename_T1 f1 f2 x) y \<longrightarrow> f1 ` FFVars_T11 x = FFVars_T11 y \<and> f2 ` FFVars_T12 x = FFVars_T12 y)
+    \<longrightarrow> rel_T1 R (permute_T1 f1 f2 x) y \<longrightarrow> f1 ` FVars_T11 x = FVars_T11 y \<and> f2 ` FVars_T12 x = FVars_T12 y)
     \<and> (\<forall>y2 f1 f2. bij f1 \<longrightarrow> |supp f1| <o |UNIV::'var set| \<longrightarrow> bij f2 \<longrightarrow> |supp f2| <o |UNIV::'tyvar set|
-    \<longrightarrow> rel_T2 R (rrename_T2 f1 f2 x2) y2 \<longrightarrow> f1 ` FFVars_T21 x2 = FFVars_T21 y2 \<and> f2 ` FFVars_T22 x2 = FFVars_T22 y2)"
+    \<longrightarrow> rel_T2 R (permute_T2 f1 f2 x2) y2 \<longrightarrow> f1 ` FVars_T21 x2 = FVars_T21 y2 \<and> f2 ` FVars_T22 x2 = FVars_T22 y2)"
     apply (rule T1.TT_plain_co_induct)
      apply (rule allI impI)+
      apply (erule rel_plain_cases)
-     apply (subst (asm) T1.rrename_cctors)
+     apply (subst (asm) T1.permute_cctors)
          apply assumption+
      apply (drule T1.TT_injects0[THEN iffD1])
      apply (erule exE conjE)+
      apply hypsubst
      apply (subst (asm) T1_pre.map_comp T1_pre.set_map, (assumption | rule supp_id_bound bij_id)+)+
      apply (unfold id_o o_id image_comp[unfolded comp_def])[1]
-     apply (subst (asm) T1.rrename_comp0s T1.FFVars_rrenames, (assumption | rule supp_id_bound bij_id)+)+
+     apply (subst (asm) T1.permute_comp0s T1.FVars_rrenames, (assumption | rule supp_id_bound bij_id)+)+
      apply (unfold image_UN[symmetric] image_set_diff[OF bij_is_inj, symmetric] id_on_Un)[1]
      apply (erule conjE)+
      apply (unfold T1_pre.mr_rel_id)[1]
@@ -1896,7 +1929,7 @@ proof -
       apply (rule impI)
         (* REPEAT_DETERM *)
       apply (rule conjI)?
-       apply (unfold T1.FFVars_cctors image_Un)[1]
+       apply (unfold T1.FVars_cctors image_Un)[1]
        apply (rule arg_cong2[of _ _ _ _ "(\<union>)"])+
            apply (rule sym)
            apply (erule T1_pre.mr_rel_set[rotated -1])
@@ -2029,7 +2062,7 @@ proof -
         (* repeated (outer) *)
         (* REPEAT_DETERM *)
       apply (rule conjI)?
-      apply (unfold T1.FFVars_cctors image_Un)[1]
+      apply (unfold T1.FVars_cctors image_Un)[1]
       apply (rule arg_cong2[of _ _ _ _ "(\<union>)"])+
           apply (rule sym)
           apply (erule T1_pre.mr_rel_set[rotated -1])
@@ -2163,14 +2196,14 @@ proof -
         (* second type, same tactic *)
     apply (rule allI impI)+
     apply (erule rel_plain_cases)
-    apply (subst (asm) T1.rrename_cctors)
+    apply (subst (asm) T1.permute_cctors)
         apply assumption+
     apply (drule T1.TT_injects0[THEN iffD1])
     apply (erule exE conjE)+
     apply hypsubst
     apply (subst (asm) T2_pre.map_comp T2_pre.set_map, (assumption | rule supp_id_bound bij_id)+)+
     apply (unfold id_o o_id image_comp[unfolded comp_def])[1]
-    apply (subst (asm) T1.rrename_comp0s T1.FFVars_rrenames, (assumption | rule supp_id_bound bij_id)+)+
+    apply (subst (asm) T1.permute_comp0s T1.FVars_rrenames, (assumption | rule supp_id_bound bij_id)+)+
     apply (unfold image_UN[symmetric] image_set_diff[OF bij_is_inj, symmetric] id_on_Un)[1]
     apply (erule conjE)+
     apply (unfold T2_pre.mr_rel_id)[1]
@@ -2183,7 +2216,7 @@ proof -
       apply (rule impI)
         (* REPEAT_DETERM *)
       apply (rule conjI)?
-       apply (unfold T1.FFVars_cctors image_Un)[1]
+       apply (unfold T1.FVars_cctors image_Un)[1]
        apply (rule arg_cong2[of _ _ _ _ "(\<union>)"])+
            apply (rule sym)
            apply (erule T2_pre.mr_rel_set[rotated -1])
@@ -2316,7 +2349,7 @@ proof -
         (* repeated (outer) *)
         (* REPEAT_DETERM *)
       apply (rule conjI)?
-      apply (unfold T1.FFVars_cctors image_Un)[1]
+      apply (unfold T1.FVars_cctors image_Un)[1]
       apply (rule arg_cong2[of _ _ _ _ "(\<union>)"])+
           apply (rule sym)
           apply (erule T2_pre.mr_rel_set[rotated -1])
@@ -2449,38 +2482,38 @@ proof -
       done
     done
   show
-    "rel_T1 R x y \<Longrightarrow> FFVars_T11 x = FFVars_T11 y"
-    "rel_T1 R x y \<Longrightarrow> FFVars_T12 x = FFVars_T12 y"
-    "rel_T2 R x2 y2 \<Longrightarrow> FFVars_T21 x2 = FFVars_T21 y2"
-    "rel_T2 R x2 y2 \<Longrightarrow> FFVars_T22 x2 = FFVars_T22 y2"
+    "rel_T1 R x y \<Longrightarrow> FVars_T11 x = FVars_T11 y"
+    "rel_T1 R x y \<Longrightarrow> FVars_T12 x = FVars_T12 y"
+    "rel_T2 R x2 y2 \<Longrightarrow> FVars_T21 x2 = FVars_T21 y2"
+    "rel_T2 R x2 y2 \<Longrightarrow> FVars_T22 x2 = FVars_T22 y2"
        apply -
       (* REPEAT_DETERM *)
        apply (insert x)[1]
        apply (erule conjE)+
        apply (erule allE)+
        apply (erule impE, rule bij_id supp_id_bound)+
-       apply (unfold image_id T1.rrename_ids)
+       apply (unfold image_id T1.permute_ids)
        apply (((erule impE, assumption) | (erule conjE)+ | assumption | erule thin_rl)+)[1]
       (* repeated *)
       apply (insert x)[1]
       apply (erule conjE)+
       apply (erule allE)+
       apply (erule impE, rule bij_id supp_id_bound)+
-      apply (unfold image_id T1.rrename_ids)
+      apply (unfold image_id T1.permute_ids)
       apply (((erule impE, assumption) | (erule conjE)+ | assumption | erule thin_rl)+)[1]
       (* repeated *)
      apply (insert x)[1]
      apply (erule conjE)+
      apply (erule allE)+
      apply (erule impE, rule bij_id supp_id_bound)+
-     apply (unfold image_id T1.rrename_ids)
+     apply (unfold image_id T1.permute_ids)
      apply (((erule impE, assumption) | (erule conjE)+ | assumption | erule thin_rl)+)[1]
       (* repeated *)
     apply (insert x)[1]
     apply (erule conjE)+
     apply (erule allE)+
     apply (erule impE, rule bij_id supp_id_bound)+
-    apply (unfold image_id T1.rrename_ids)
+    apply (unfold image_id T1.permute_ids)
     apply (((erule impE, assumption) | (erule conjE)+ | assumption | erule thin_rl)+)[1]
     done
 qed
@@ -2489,16 +2522,16 @@ qed
 (*********** MRBNF Axiom Proofs ************)
 (* required for other proofs, ie needed as `thm` *)
 
-lemma FFVars_vvsubstss:
+lemma FVars_vvsubstss:
   fixes f1::"'var::{var_T1_pre,var_T2_pre} \<Rightarrow> 'var" and f2::"'tyvar::{var_T1_pre,var_T2_pre} \<Rightarrow> 'tyvar" and f3::"'a::{var_T1_pre,var_T2_pre} \<Rightarrow> 'a" and f4::"'b \<Rightarrow> 'c"
   assumes f_prems: "|supp f1| <o |UNIV::'var set|" "|supp f2| <o |UNIV::'tyvar set|" "|supp f3| <o |UNIV::'a set|"
-  shows "FFVars_T11 (vvsubst_T1 f1 f2 f3 f4 x) = f1 ` FFVars_T11 x"
-    "FFVars_T12 (vvsubst_T1 f1 f2 f3 f4 x) = f2 ` FFVars_T12 x"
-    "FFVars_T21 (vvsubst_T2 f1 f2 f3 f4 y) = f1 ` FFVars_T21 y"
-    "FFVars_T22 (vvsubst_T2 f1 f2 f3 f4 y) = f2 ` FFVars_T22 y"
+  shows "FVars_T11 (vvsubst_T1 f1 f2 f3 f4 x) = f1 ` FVars_T11 x"
+    "FVars_T12 (vvsubst_T1 f1 f2 f3 f4 x) = f2 ` FVars_T12 x"
+    "FVars_T21 (vvsubst_T2 f1 f2 f3 f4 y) = f1 ` FVars_T21 y"
+    "FVars_T22 (vvsubst_T2 f1 f2 f3 f4 y) = f2 ` FVars_T22 y"
 proof -
-  have x: "((FFVars_T11 (vvsubst_T1 f1 f2 f3 f4 x) = f1 ` FFVars_T11 x) \<and> (FFVars_T12 (vvsubst_T1 f1 f2 f3 f4 x) = f2 ` FFVars_T12 x))
-      \<and> ((FFVars_T21 (vvsubst_T2 f1 f2 f3 f4 y) = f1 ` FFVars_T21 y) \<and> (FFVars_T22 (vvsubst_T2 f1 f2 f3 f4 y) = f2 ` FFVars_T22 y))"
+  have x: "((FVars_T11 (vvsubst_T1 f1 f2 f3 f4 x) = f1 ` FVars_T11 x) \<and> (FVars_T12 (vvsubst_T1 f1 f2 f3 f4 x) = f2 ` FVars_T12 x))
+      \<and> ((FVars_T21 (vvsubst_T2 f1 f2 f3 f4 y) = f1 ` FVars_T21 y) \<and> (FVars_T22 (vvsubst_T2 f1 f2 f3 f4 y) = f2 ` FVars_T22 y))"
     apply (rule T1.TT_fresh_co_induct[of _ _ _ _ x y, rotated 2])
        apply (rule conjI)
         apply (subst vvsubst_cctor_1)
@@ -2516,7 +2549,7 @@ proof -
       (* END REPEAT_DETERM *)
          apply assumption
 
-        apply (unfold T1.FFVars_cctors image_Un image_UN)
+        apply (unfold T1.FVars_cctors image_Un image_UN)
         apply (subst T1_pre.set_map, (rule f_prems supp_id_bound bij_id)+)+
         apply (rule arg_cong2[of _ _ _ _ "(\<union>)"])+
             apply (rule refl)
@@ -2564,7 +2597,7 @@ proof -
       (* END REPEAT_DETERM *)
         apply assumption
 
-       apply (unfold T1.FFVars_cctors image_Un image_UN)
+       apply (unfold T1.FVars_cctors image_Un image_UN)
        apply (subst T1_pre.set_map, (rule f_prems supp_id_bound bij_id)+)+
        apply (rule arg_cong2[of _ _ _ _ "(\<union>)"])+
            apply (rule refl)
@@ -2614,7 +2647,7 @@ proof -
       (* END REPEAT_DETERM *)
         apply assumption
 
-       apply (unfold T1.FFVars_cctors image_Un image_UN)
+       apply (unfold T1.FVars_cctors image_Un image_UN)
        apply (subst T2_pre.set_map, (rule f_prems supp_id_bound bij_id)+)+
        apply (rule arg_cong2[of _ _ _ _ "(\<union>)"])+
            apply (rule refl)+
@@ -2662,7 +2695,7 @@ proof -
       (* END REPEAT_DETERM *)
        apply assumption
 
-      apply (unfold T1.FFVars_cctors image_Un image_UN)
+      apply (unfold T1.FVars_cctors image_Un image_UN)
       apply (subst T2_pre.set_map, (rule f_prems supp_id_bound bij_id)+)+
       apply (rule arg_cong2[of _ _ _ _ "(\<union>)"])+
           apply (rule refl)+
@@ -2697,22 +2730,22 @@ proof -
 
      apply (rule iffD2[OF imsupp_supp_bound] infinite_UNIV f_prems)+
     done
-  show "FFVars_T11 (vvsubst_T1 f1 f2 f3 f4 x) = f1 ` FFVars_T11 x"
+  show "FVars_T11 (vvsubst_T1 f1 f2 f3 f4 x) = f1 ` FVars_T11 x"
     apply (insert x)
     apply (erule conjE)+
     apply assumption
     done
-  show "FFVars_T12 (vvsubst_T1 f1 f2 f3 f4 x) = f2 ` FFVars_T12 x"
+  show "FVars_T12 (vvsubst_T1 f1 f2 f3 f4 x) = f2 ` FVars_T12 x"
     apply (insert x)
     apply (erule conjE)+
     apply assumption
     done
-  show "FFVars_T21 (vvsubst_T2 f1 f2 f3 f4 y) = f1 ` FFVars_T21 y"
+  show "FVars_T21 (vvsubst_T2 f1 f2 f3 f4 y) = f1 ` FVars_T21 y"
     apply (insert x)
     apply (erule conjE)+
     apply assumption
     done
-  show "FFVars_T22 (vvsubst_T2 f1 f2 f3 f4 y) = f2 ` FFVars_T22 y"
+  show "FVars_T22 (vvsubst_T2 f1 f2 f3 f4 y) = f2 ` FVars_T22 y"
     apply (insert x)
     apply (erule conjE)+
     apply assumption
@@ -2953,7 +2986,7 @@ proof -
           apply (subst noclash_T1_def)
           apply (subst T1_pre.set_map, (rule f_prems supp_id_bound bij_id)+)+
           apply (unfold image_id image_comp[unfolded comp_def])
-          apply (subst FFVars_vvsubstss, (rule f_prems)+)+
+          apply (subst FVars_vvsubstss, (rule f_prems)+)+
           apply (unfold image_UN[symmetric] image_Un[symmetric])
         (* REPEAT_DETERM *)
           apply (subst Int_image_imsupp)
@@ -3057,7 +3090,7 @@ proof -
          apply (subst noclash_T2_def)
          apply (subst T2_pre.set_map, (rule f_prems supp_id_bound bij_id)+)+
          apply (unfold image_id image_comp[unfolded comp_def])
-         apply (subst FFVars_vvsubstss, (rule f_prems)+)+
+         apply (subst FVars_vvsubstss, (rule f_prems)+)+
          apply (unfold image_UN[symmetric] image_Un[symmetric])
         (* REPEAT_DETERM *)
          apply (subst Int_image_imsupp)
@@ -3155,13 +3188,13 @@ lemma vvsubst_cong:
   assumes f_prems: "|supp f1| <o |UNIV::'var set|" "|supp f2| <o |UNIV::'tyvar set|" "|supp f3| <o |UNIV::'a set|"
     and g_prems: "|supp g1| <o |UNIV::'var set|" "|supp g2| <o |UNIV::'tyvar set|" "|supp g3| <o |UNIV::'a set|"
   shows
-    "(\<And>a. a \<in> FFVars_T11 x \<Longrightarrow> f1 a = g1 a) \<Longrightarrow> (\<And>a. a \<in> FFVars_T12 x \<Longrightarrow> f2 a = g2 a) \<Longrightarrow> (\<And>a. a \<in> set3_T1 x \<Longrightarrow> f3 a = g3 a) \<Longrightarrow> (\<And>a. a \<in> set4_T1 x \<Longrightarrow> f4 a = g4 a) \<Longrightarrow> vvsubst_T1 f1 f2 f3 f4 x = vvsubst_T1 g1 g2 g3 g4 x"
-    "(\<And>a. a \<in> FFVars_T21 y \<Longrightarrow> f1 a = g1 a) \<Longrightarrow> (\<And>a. a \<in> FFVars_T22 y \<Longrightarrow> f2 a = g2 a) \<Longrightarrow> (\<And>a. a \<in> set3_T2 y \<Longrightarrow> f3 a = g3 a) \<Longrightarrow> (\<And>a. a \<in> set4_T2 y \<Longrightarrow> f4 a = g4 a) \<Longrightarrow> vvsubst_T2 f1 f2 f3 f4 y = vvsubst_T2 g1 g2 g3 g4 y"
+    "(\<And>a. a \<in> FVars_T11 x \<Longrightarrow> f1 a = g1 a) \<Longrightarrow> (\<And>a. a \<in> FVars_T12 x \<Longrightarrow> f2 a = g2 a) \<Longrightarrow> (\<And>a. a \<in> set3_T1 x \<Longrightarrow> f3 a = g3 a) \<Longrightarrow> (\<And>a. a \<in> set4_T1 x \<Longrightarrow> f4 a = g4 a) \<Longrightarrow> vvsubst_T1 f1 f2 f3 f4 x = vvsubst_T1 g1 g2 g3 g4 x"
+    "(\<And>a. a \<in> FVars_T21 y \<Longrightarrow> f1 a = g1 a) \<Longrightarrow> (\<And>a. a \<in> FVars_T22 y \<Longrightarrow> f2 a = g2 a) \<Longrightarrow> (\<And>a. a \<in> set3_T2 y \<Longrightarrow> f3 a = g3 a) \<Longrightarrow> (\<And>a. a \<in> set4_T2 y \<Longrightarrow> f4 a = g4 a) \<Longrightarrow> vvsubst_T2 f1 f2 f3 f4 y = vvsubst_T2 g1 g2 g3 g4 y"
 proof -
-  have x: "((\<forall>a. a \<in> FFVars_T11 x \<longrightarrow> f1 a = g1 a) \<longrightarrow>
-    (\<forall>a. a \<in> FFVars_T12 x \<longrightarrow> f2 a = g2 a) \<longrightarrow> (\<forall>a. a \<in> set3_T1 x \<longrightarrow> f3 a = g3 a) \<longrightarrow> (\<forall>a. a \<in> set4_T1 x \<longrightarrow> f4 a = g4 a) \<longrightarrow> vvsubst_T1 f1 f2 f3 f4 x = vvsubst_T1 g1 g2 g3 g4 x)
-    \<and> ((\<forall>a. a \<in> FFVars_T21 y \<longrightarrow> f1 a = g1 a) \<longrightarrow>
-    (\<forall>a. a \<in> FFVars_T22 y \<longrightarrow> f2 a = g2 a) \<longrightarrow> (\<forall>a. a \<in> set3_T2 y \<longrightarrow> f3 a = g3 a) \<longrightarrow> (\<forall>a. a \<in> set4_T2 y \<longrightarrow> f4 a = g4 a) \<longrightarrow> vvsubst_T2 f1 f2 f3 f4 y = vvsubst_T2 g1 g2 g3 g4 y)"
+  have x: "((\<forall>a. a \<in> FVars_T11 x \<longrightarrow> f1 a = g1 a) \<longrightarrow>
+    (\<forall>a. a \<in> FVars_T12 x \<longrightarrow> f2 a = g2 a) \<longrightarrow> (\<forall>a. a \<in> set3_T1 x \<longrightarrow> f3 a = g3 a) \<longrightarrow> (\<forall>a. a \<in> set4_T1 x \<longrightarrow> f4 a = g4 a) \<longrightarrow> vvsubst_T1 f1 f2 f3 f4 x = vvsubst_T1 g1 g2 g3 g4 x)
+    \<and> ((\<forall>a. a \<in> FVars_T21 y \<longrightarrow> f1 a = g1 a) \<longrightarrow>
+    (\<forall>a. a \<in> FVars_T22 y \<longrightarrow> f2 a = g2 a) \<longrightarrow> (\<forall>a. a \<in> set3_T2 y \<longrightarrow> f3 a = g3 a) \<longrightarrow> (\<forall>a. a \<in> set4_T2 y \<longrightarrow> f4 a = g4 a) \<longrightarrow> vvsubst_T2 f1 f2 f3 f4 y = vvsubst_T2 g1 g2 g3 g4 y)"
     apply (rule T1.TT_fresh_co_induct[of _ _ _ _ x y, rotated 2])
        apply (rule allI impI)+
        apply (rule trans)
@@ -3211,7 +3244,7 @@ proof -
     subgoal premises prems
       apply (rule T1_pre.map_cong0)
                           apply (rule f_prems g_prems supp_id_bound bij_id)+
-               apply (rule prems, erule T1.FFVars_intros)+
+               apply (rule prems, erule T1.FVars_intros)+
              apply (rule prems)
              apply (unfold set3_T1_simp)[1]
              apply (rule UnI1)+
@@ -3224,10 +3257,10 @@ proof -
 
          apply (frule prems)
              apply (rule prems)
-             apply (erule T1.FFVars_intros)
+             apply (erule T1.FVars_intros)
              apply assumption
             apply (rule prems)
-            apply (erule T1.FFVars_intros)
+            apply (erule T1.FVars_intros)
             apply assumption
            apply (rule prems)
            apply (erule set3_T1_intros)
@@ -3239,7 +3272,7 @@ proof -
         apply (frule prems)
             apply (rule case_split[of "_ \<in> _", rotated])
              apply (rule prems)
-             apply (erule T1.FFVars_intros)
+             apply (erule T1.FVars_intros)
               apply assumption
              apply assumption
             apply (drule prems(5-10))
@@ -3252,7 +3285,7 @@ proof -
 
            apply (rule case_split[of "_ \<in> _", rotated])
             apply (rule prems)
-            apply (erule T1.FFVars_intros)
+            apply (erule T1.FVars_intros)
              apply assumption
             apply assumption
            apply (drule prems(5-10))
@@ -3274,10 +3307,10 @@ proof -
 
        apply (frule prems)
            apply (rule prems)
-           apply (erule T1.FFVars_intros)
+           apply (erule T1.FVars_intros)
            apply assumption
           apply (rule prems)
-          apply (erule T1.FFVars_intros)
+          apply (erule T1.FVars_intros)
           apply assumption
          apply (rule prems)
          apply (erule set3_T1_intros)
@@ -3290,7 +3323,7 @@ proof -
       apply (frule prems)
           apply (rule case_split[of "_ \<in> _", rotated])
            apply (rule prems)
-           apply (erule T1.FFVars_intros)
+           apply (erule T1.FVars_intros)
             apply assumption
            apply assumption
           apply (drule prems(5-10))
@@ -3302,7 +3335,7 @@ proof -
           apply (erule not_in_imsupp_same)
 
          apply (rule prems)
-         apply (erule T1.FFVars_intros)
+         apply (erule T1.FVars_intros)
          apply assumption
         apply (rule prems)
         apply (erule set3_T1_intros)
@@ -3360,7 +3393,7 @@ proof -
     subgoal premises prems
       apply (rule T2_pre.map_cong0)
                           apply (rule f_prems g_prems supp_id_bound bij_id)+
-               apply (rule prems, erule T1.FFVars_intros)+
+               apply (rule prems, erule T1.FVars_intros)+
              apply (rule prems)
              apply (unfold set3_T2_simp)[1]
              apply (rule UnI1)+
@@ -3373,10 +3406,10 @@ proof -
 
          apply (frule prems)
              apply (rule prems)
-             apply (erule T1.FFVars_intros)
+             apply (erule T1.FVars_intros)
              apply assumption
             apply (rule prems)
-            apply (erule T1.FFVars_intros)
+            apply (erule T1.FVars_intros)
             apply assumption
            apply (rule prems)
            apply (erule set3_T2_intros)
@@ -3389,7 +3422,7 @@ proof -
         apply (frule prems)
             apply (rule case_split[of "_ \<in> _", rotated])
              apply (rule prems)
-             apply (erule T1.FFVars_intros)
+             apply (erule T1.FVars_intros)
               apply assumption
              apply assumption
             apply (drule prems(5-10))
@@ -3402,7 +3435,7 @@ proof -
 
            apply (rule case_split[of "_ \<in> _", rotated])
             apply (rule prems)
-            apply (erule T1.FFVars_intros)
+            apply (erule T1.FVars_intros)
              apply assumption
             apply assumption
            apply (drule prems(5-10))
@@ -3424,10 +3457,10 @@ proof -
 
        apply (frule prems)
            apply (rule prems)
-           apply (erule T1.FFVars_intros)
+           apply (erule T1.FVars_intros)
            apply assumption
           apply (rule prems)
-          apply (erule T1.FFVars_intros)
+          apply (erule T1.FVars_intros)
           apply assumption
          apply (rule prems)
          apply (erule set3_T2_intros)
@@ -3440,7 +3473,7 @@ proof -
       apply (frule prems)
           apply (rule case_split[of "_ \<in> _", rotated])
            apply (rule prems)
-           apply (erule T1.FFVars_intros)
+           apply (erule T1.FVars_intros)
             apply assumption
            apply assumption
           apply (drule prems(5-10))
@@ -3452,7 +3485,7 @@ proof -
           apply (erule not_in_imsupp_same)
 
          apply (rule prems)
-         apply (erule T1.FFVars_intros)
+         apply (erule T1.FVars_intros)
          apply assumption
         apply (rule prems)
         apply (erule set3_T2_intros)
@@ -3466,8 +3499,8 @@ proof -
      apply (rule T1_pre.Un_bound iffD2[OF imsupp_supp_bound] infinite_UNIV f_prems g_prems)+
     done
 
-  show "(\<And>a. a \<in> FFVars_T11 x \<Longrightarrow> f1 a = g1 a) \<Longrightarrow>
-    (\<And>a. a \<in> FFVars_T12 x \<Longrightarrow> f2 a = g2 a) \<Longrightarrow> (\<And>a. a \<in> set3_T1 x \<Longrightarrow> f3 a = g3 a) \<Longrightarrow> (\<And>a. a \<in> set4_T1 x \<Longrightarrow> f4 a = g4 a) \<Longrightarrow> vvsubst_T1 f1 f2 f3 f4 x = vvsubst_T1 g1 g2 g3 g4 x"
+  show "(\<And>a. a \<in> FVars_T11 x \<Longrightarrow> f1 a = g1 a) \<Longrightarrow>
+    (\<And>a. a \<in> FVars_T12 x \<Longrightarrow> f2 a = g2 a) \<Longrightarrow> (\<And>a. a \<in> set3_T1 x \<Longrightarrow> f3 a = g3 a) \<Longrightarrow> (\<And>a. a \<in> set4_T1 x \<Longrightarrow> f4 a = g4 a) \<Longrightarrow> vvsubst_T1 f1 f2 f3 f4 x = vvsubst_T1 g1 g2 g3 g4 x"
     apply (insert x)
     apply (erule conjE)+
     apply (unfold imp_conjL[symmetric])
@@ -3486,7 +3519,7 @@ proof -
     apply assumption
     done
 
-  show "(\<And>a. a \<in> FFVars_T21 y \<Longrightarrow> f1 a = g1 a) \<Longrightarrow> (\<And>a. a \<in> FFVars_T22 y \<Longrightarrow> f2 a = g2 a) \<Longrightarrow>
+  show "(\<And>a. a \<in> FVars_T21 y \<Longrightarrow> f1 a = g1 a) \<Longrightarrow> (\<And>a. a \<in> FVars_T22 y \<Longrightarrow> f2 a = g2 a) \<Longrightarrow>
     (\<And>a. a \<in> set3_T2 y \<Longrightarrow> f3 a = g3 a) \<Longrightarrow> (\<And>a. a \<in> set4_T2 y \<Longrightarrow> f4 a = g4 a) \<Longrightarrow> vvsubst_T2 f1 f2 f3 f4 y = vvsubst_T2 g1 g2 g3 g4 y"
     apply (insert x)
     apply (erule conjE)+
@@ -3512,10 +3545,10 @@ lemma rel_OO_mono:
   "(rel_T2 R :: ('var, 'tyvar, 'a, 'b) T2 \<Rightarrow> _) OO rel_T2 S \<le> rel_T2 (R OO S)"
 proof -
   have x: "(\<forall>R' (x::('var, 'tyvar, 'a, 'b) T1) z. R' = R OO S \<and> (\<exists>y f1 f2 x'. bij f1 \<and> |supp f1| <o |UNIV::'var set|
-    \<and> bij f2 \<and> |supp f2| <o |UNIV::'tyvar set| \<and> x = rrename_T1 f1 f2 x' \<and> rel_T1 R x y \<and> rel_T1 S y z) \<longrightarrow>
+    \<and> bij f2 \<and> |supp f2| <o |UNIV::'tyvar set| \<and> x = permute_T1 f1 f2 x' \<and> rel_T1 R x y \<and> rel_T1 S y z) \<longrightarrow>
     rel_T1 R' x z) \<and>
   (\<forall>R' (x::('var, 'tyvar, 'a, 'b) T2) z. R' = R OO S \<and> (\<exists>y f1 f2 x'. bij f1 \<and> |supp f1| <o |UNIV::'var set|
-    \<and> bij f2 \<and> |supp f2| <o |UNIV::'tyvar set| \<and> x = rrename_T2 f1 f2 x' \<and> rel_T2 R x y \<and> rel_T2 S y z) \<longrightarrow>
+    \<and> bij f2 \<and> |supp f2| <o |UNIV::'tyvar set| \<and> x = permute_T2 f1 f2 x' \<and> rel_T2 R x y \<and> rel_T2 S y z) \<longrightarrow>
     rel_T2 R' x z)"
     apply (rule rel_T1_rel_T2.coinduct)
      apply (erule conjE exE)+
@@ -3524,9 +3557,9 @@ proof -
      apply hypsubst
      apply (unfold triv_forall_equality)
     subgoal for f1 f2 x'2 x' y' y'2 z'
-      apply (drule arg_cong[of _ _ "rrename_T1 (inv f1) (inv f2)"])
-      apply (subst (asm) T1.rrename_comps inv_o_simp1 T1.rrename_cctors, (assumption | rule bij_imp_bij_inv supp_inv_bound)+)+
-      apply (unfold T1.rrename_ids)
+      apply (drule arg_cong[of _ _ "permute_T1 (inv f1) (inv f2)"])
+      apply (subst (asm) T1.permute_comps inv_o_simp1 T1.permute_cctors, (assumption | rule bij_imp_bij_inv supp_inv_bound)+)+
+      apply (unfold T1.permute_ids)
       apply hypsubst_thin
       apply (drule T1.TT_injects0[THEN iffD1])
       apply (erule conjE exE)+
@@ -3542,12 +3575,12 @@ proof -
       apply (rule conjI)
        apply (rule refl)
       apply (rule conjI)
-       apply (subst T1.rrename_cctors[symmetric])
+       apply (subst T1.permute_cctors[symmetric])
            apply (rule bij_imp_bij_inv supp_inv_bound | assumption)+
        apply (rule trans)
-        apply (rule T1.rrename_comps)
+        apply (rule T1.permute_comps)
                apply (rule bij_imp_bij_inv supp_inv_bound | assumption)+
-       apply (rule T1.rrename_cong_ids)
+       apply (rule T1.permute_cong_ids)
             apply (rule bij_comp supp_comp_bound bij_imp_bij_inv supp_inv_bound infinite_UNIV | assumption)+
         apply (subst inv_o_simp2, assumption, rule id_apply)+
       apply (rule conjI)
@@ -3571,7 +3604,7 @@ proof -
                           apply (rule conjI[rotated])+
                           apply assumption
                           apply (assumption | (rule rel_rrename[THEN iffD2], (assumption | rule bij_id supp_id_bound)+))
-                          apply (rule refl T1.rrename_ids[symmetric])
+                          apply (rule refl T1.permute_ids[symmetric])
                           apply (rule supp_id_bound bij_id | assumption)+
         (* repeated *)
                           apply ((rule ballI impI)+)?
@@ -3585,7 +3618,7 @@ proof -
                           apply (rule conjI[rotated])+
                           apply assumption
                           apply (assumption | (rule rel_rrename[THEN iffD2], (assumption | rule bij_id supp_id_bound)+))
-                          apply (rule refl T1.rrename_ids[symmetric])
+                          apply (rule refl T1.permute_ids[symmetric])
                           apply (rule supp_id_bound bij_id | assumption)+
         (* repeated *)
                           apply ((rule ballI impI)+)?
@@ -3599,7 +3632,7 @@ proof -
                           apply (rule conjI[rotated])+
                           apply assumption
                           apply (assumption | (rule rel_rrename[THEN iffD2], (assumption | rule bij_id supp_id_bound)+))
-                          apply (rule refl T1.rrename_ids[symmetric])
+                          apply (rule refl T1.permute_ids[symmetric])
                           apply (rule supp_id_bound bij_id | assumption)+
         (* repeated *)
                           apply ((rule ballI impI)+)?
@@ -3613,7 +3646,7 @@ proof -
                           apply (rule conjI[rotated])+
                           apply assumption
                           apply (assumption | (rule rel_rrename[THEN iffD2], (assumption | rule bij_id supp_id_bound)+))
-                          apply (rule refl T1.rrename_ids[symmetric])
+                          apply (rule refl T1.permute_ids[symmetric])
                           apply (rule supp_id_bound bij_id | assumption)+
         (* END REPEAT_DETERM *)
         (* REPEAT_DETERM *)
@@ -3669,9 +3702,9 @@ proof -
     apply hypsubst
     apply (unfold triv_forall_equality)
     subgoal for f1 f2 x'2 x' y' y'2 z'
-      apply (drule arg_cong[of _ _ "rrename_T2 (inv f1) (inv f2)"])
-      apply (subst (asm) T1.rrename_comps inv_o_simp1 T1.rrename_cctors, (assumption | rule bij_imp_bij_inv supp_inv_bound)+)+
-      apply (unfold T1.rrename_ids)
+      apply (drule arg_cong[of _ _ "permute_T2 (inv f1) (inv f2)"])
+      apply (subst (asm) T1.permute_comps inv_o_simp1 T1.permute_cctors, (assumption | rule bij_imp_bij_inv supp_inv_bound)+)+
+      apply (unfold T1.permute_ids)
       apply hypsubst_thin
       apply (drule T1.TT_injects0[THEN iffD1])
       apply (erule conjE exE)+
@@ -3687,12 +3720,12 @@ proof -
       apply (rule conjI)
        apply (rule refl)
       apply (rule conjI)
-       apply (subst T1.rrename_cctors[symmetric])
+       apply (subst T1.permute_cctors[symmetric])
            apply (rule bij_imp_bij_inv supp_inv_bound | assumption)+
        apply (rule trans)
-        apply (rule T1.rrename_comps)
+        apply (rule T1.permute_comps)
                apply (rule bij_imp_bij_inv supp_inv_bound | assumption)+
-       apply (rule T1.rrename_cong_ids)
+       apply (rule T1.permute_cong_ids)
             apply (rule bij_comp supp_comp_bound bij_imp_bij_inv supp_inv_bound infinite_UNIV | assumption)+
         apply (subst inv_o_simp2, assumption, rule id_apply)+
       apply (rule conjI)
@@ -3716,7 +3749,7 @@ proof -
                           apply (rule conjI[rotated])+
                           apply assumption
                           apply (assumption | (rule rel_rrename[THEN iffD2], (assumption | rule bij_id supp_id_bound)+))
-                          apply (rule refl T1.rrename_ids[symmetric])
+                          apply (rule refl T1.permute_ids[symmetric])
                           apply (rule supp_id_bound bij_id | assumption)+
         (* repeated *)
                           apply ((rule ballI impI)+)?
@@ -3730,7 +3763,7 @@ proof -
                           apply (rule conjI[rotated])+
                           apply assumption
                           apply (assumption | (rule rel_rrename[THEN iffD2], (assumption | rule bij_id supp_id_bound)+))
-                          apply (rule refl T1.rrename_ids[symmetric])
+                          apply (rule refl T1.permute_ids[symmetric])
                           apply (rule supp_id_bound bij_id | assumption)+
         (* repeated *)
                           apply ((rule ballI impI)+)?
@@ -3744,7 +3777,7 @@ proof -
                           apply (rule conjI[rotated])+
                           apply assumption
                           apply (assumption | (rule rel_rrename[THEN iffD2], (assumption | rule bij_id supp_id_bound)+))
-                          apply (rule refl T1.rrename_ids[symmetric])
+                          apply (rule refl T1.permute_ids[symmetric])
                           apply (rule supp_id_bound bij_id | assumption)+
         (* repeated *)
                           apply ((rule ballI impI)+)?
@@ -3758,7 +3791,7 @@ proof -
                           apply (rule conjI[rotated])+
                           apply assumption
                           apply (assumption | (rule rel_rrename[THEN iffD2], (assumption | rule bij_id supp_id_bound)+))
-                          apply (rule refl T1.rrename_ids[symmetric])
+                          apply (rule refl T1.permute_ids[symmetric])
                           apply (rule supp_id_bound bij_id | assumption)+
         (* END REPEAT_DETERM *)
         (* REPEAT_DETERM *)
@@ -3820,7 +3853,7 @@ proof -
       apply (erule mp)
       apply (rule conjI)
        apply (rule refl)
-      apply (rule exI conjI bij_id supp_id_bound T1.rrename_ids[symmetric] | assumption)+
+      apply (rule exI conjI bij_id supp_id_bound T1.permute_ids[symmetric] | assumption)+
       done
     subgoal
       apply (rule predicate2I)
@@ -3830,7 +3863,7 @@ proof -
       apply (erule mp)
       apply (rule conjI)
        apply (rule refl)
-      apply (rule exI conjI bij_id supp_id_bound T1.rrename_ids[symmetric] | assumption)+
+      apply (rule exI conjI bij_id supp_id_bound T1.permute_ids[symmetric] | assumption)+
       done
     done
 qed
@@ -3896,7 +3929,7 @@ proof -
       apply hypsubst
       apply (subst (asm) T1_pre.map_comp T1_pre.set_map, (rule assms bij_id supp_id_bound | assumption)+)+
       apply (unfold id_o o_id image_id image_comp[unfolded comp_def])
-      apply (subst (asm) FFVars_vvsubstss, (rule assms | assumption)+)+
+      apply (subst (asm) FVars_vvsubstss, (rule assms | assumption)+)+
       apply (unfold image_UN[symmetric] T1_pre.mr_rel_id)
       apply (drule iffD1[OF T1_pre.mr_rel_map(1), rotated -1])
                     apply (rule assms supp_id_bound bij_id | assumption)+
@@ -4164,7 +4197,7 @@ proof -
           (* REPEAT_DETERM *)
            apply (rule Diff_mono[OF _ subset_refl])
            apply (unfold image_comp comp_def)[1]
-           apply (subst FFVars_vvsubstss)
+           apply (subst FVars_vvsubstss)
               apply (rule assms | assumption)+
            apply (unfold image_UN[symmetric])
            apply (rule image_mono)
@@ -4181,13 +4214,13 @@ proof -
            apply (rotate_tac -2)
            apply (rule trans[rotated])
             apply (erule arg_cong)
-           apply (subst FFVars_vvsubstss)
+           apply (subst FVars_vvsubstss)
               apply (rule supp_id_bound bij_id)+
            apply (rule image_id[symmetric])
           (* repeated *)
            apply (rule Diff_mono[OF _ subset_refl])
-           apply (unfold image_comp comp_assoc[symmetric] comp_def[of FFVars_T11] comp_def[of FFVars_T21])[1]
-           apply (subst FFVars_vvsubstss)
+           apply (unfold image_comp comp_assoc[symmetric] comp_def[of FVars_T11] comp_def[of FVars_T21])[1]
+           apply (subst FVars_vvsubstss)
               apply (rule assms | assumption)+
            apply (subst comp_def)
            apply (unfold image_UN[symmetric])
@@ -4205,7 +4238,7 @@ proof -
            apply (rotate_tac -2)
            apply (rule trans[rotated])
             apply (erule arg_cong)
-           apply (subst FFVars_vvsubstss)
+           apply (subst FVars_vvsubstss)
               apply (rule supp_id_bound bij_id)+
            apply (rule image_id[symmetric])
           (* END REPEAT_DETERM *)
@@ -4218,8 +4251,8 @@ proof -
           apply ((rule Un_mono)+)?
           (* REPEAT_DETERM *)
            apply (rule Diff_mono[OF _ subset_refl])
-           apply (unfold image_comp comp_assoc[symmetric] comp_def[of FFVars_T11] comp_def[of FFVars_T21] comp_def[of FFVars_T12] comp_def[of FFVars_T22])[1]
-           apply (subst FFVars_vvsubstss)
+           apply (unfold image_comp comp_assoc[symmetric] comp_def[of FVars_T11] comp_def[of FVars_T21] comp_def[of FVars_T12] comp_def[of FVars_T22])[1]
+           apply (subst FVars_vvsubstss)
               apply (rule assms | assumption)+
            apply (subst comp_def)
            apply (unfold image_UN[symmetric])
@@ -4237,7 +4270,7 @@ proof -
            apply (rotate_tac -2)
            apply (rule trans[rotated])
             apply (erule arg_cong)
-           apply (subst FFVars_vvsubstss)
+           apply (subst FVars_vvsubstss)
               apply (rule supp_id_bound bij_id)+
            apply (rule image_id[symmetric])
           (* END REPEAT_DETERM *)
@@ -4325,7 +4358,7 @@ proof -
               apply (erule arg_cong)
              apply (rule sym)
              apply (rule trans)
-              apply (rule FFVars_vvsubstss)
+              apply (rule FVars_vvsubstss)
                 apply (rule supp_id_bound bij_id)+
              apply (rule image_id)
         (* repeated *)
@@ -4349,7 +4382,7 @@ proof -
               apply (erule arg_cong)
              apply (rule sym)
              apply (rule trans)
-              apply (rule FFVars_vvsubstss)
+              apply (rule FVars_vvsubstss)
                 apply (rule supp_id_bound bij_id)+
             apply (rule image_id)
           (* END REPEAT_DETERM *)
@@ -4376,7 +4409,7 @@ proof -
               apply (erule arg_cong)
              apply (rule sym)
              apply (rule trans)
-              apply (rule FFVars_vvsubstss)
+              apply (rule FVars_vvsubstss)
                 apply (rule supp_id_bound bij_id)+
           apply (rule image_id)
         (* repeated *)
@@ -4401,7 +4434,7 @@ proof -
               apply (erule arg_cong)
              apply (rule sym)
              apply (rule trans)
-              apply (rule FFVars_vvsubstss)
+              apply (rule FVars_vvsubstss)
                 apply (rule supp_id_bound bij_id)+
           apply (rule image_id)
         (* repeated *)
@@ -4425,7 +4458,7 @@ proof -
               apply (erule arg_cong)
              apply (rule sym)
              apply (rule trans)
-              apply (rule FFVars_vvsubstss)
+              apply (rule FVars_vvsubstss)
                 apply (rule supp_id_bound bij_id)+
           apply (rule image_id)
         (* END REPEAT_DETERM *)
@@ -4458,7 +4491,7 @@ proof -
       apply hypsubst
       apply (subst (asm) T2_pre.map_comp T2_pre.set_map, (rule assms bij_id supp_id_bound | assumption)+)+
       apply (unfold id_o o_id image_id image_comp[unfolded comp_def])
-      apply (subst (asm) FFVars_vvsubstss, (rule assms | assumption)+)+
+      apply (subst (asm) FVars_vvsubstss, (rule assms | assumption)+)+
       apply (unfold image_UN[symmetric] T2_pre.mr_rel_id)
       apply (drule iffD1[OF T2_pre.mr_rel_map(1), rotated -1])
                     apply (rule assms supp_id_bound bij_id | assumption)+
@@ -4726,7 +4759,7 @@ proof -
           (* REPEAT_DETERM *)
            apply (rule Diff_mono[OF _ subset_refl])
            apply (unfold image_comp comp_def)[1]
-           apply (subst FFVars_vvsubstss)
+           apply (subst FVars_vvsubstss)
               apply (rule assms | assumption)+
            apply (unfold image_UN[symmetric])
            apply (rule image_mono)
@@ -4743,13 +4776,13 @@ proof -
            apply (rotate_tac -2)
            apply (rule trans[rotated])
             apply (erule arg_cong)
-           apply (subst FFVars_vvsubstss)
+           apply (subst FVars_vvsubstss)
               apply (rule supp_id_bound bij_id)+
            apply (rule image_id[symmetric])
           (* repeated *)
            apply (rule Diff_mono[OF _ subset_refl])
-           apply (unfold image_comp comp_assoc[symmetric] comp_def[of FFVars_T11] comp_def[of FFVars_T21])[1]
-           apply (subst FFVars_vvsubstss)
+           apply (unfold image_comp comp_assoc[symmetric] comp_def[of FVars_T11] comp_def[of FVars_T21])[1]
+           apply (subst FVars_vvsubstss)
               apply (rule assms | assumption)+
            apply (subst comp_def)
            apply (unfold image_UN[symmetric])
@@ -4767,7 +4800,7 @@ proof -
            apply (rotate_tac -2)
            apply (rule trans[rotated])
             apply (erule arg_cong)
-           apply (subst FFVars_vvsubstss)
+           apply (subst FVars_vvsubstss)
               apply (rule supp_id_bound bij_id)+
            apply (rule image_id[symmetric])
           (* END REPEAT_DETERM *)
@@ -4780,8 +4813,8 @@ proof -
           apply ((rule Un_mono)+)?
           (* REPEAT_DETERM *)
            apply (rule Diff_mono[OF _ subset_refl])
-           apply (unfold image_comp comp_assoc[symmetric] comp_def[of FFVars_T11] comp_def[of FFVars_T21] comp_def[of FFVars_T12] comp_def[of FFVars_T22])[1]
-           apply (subst FFVars_vvsubstss)
+           apply (unfold image_comp comp_assoc[symmetric] comp_def[of FVars_T11] comp_def[of FVars_T21] comp_def[of FVars_T12] comp_def[of FVars_T22])[1]
+           apply (subst FVars_vvsubstss)
               apply (rule assms | assumption)+
            apply (subst comp_def)
            apply (unfold image_UN[symmetric])
@@ -4799,7 +4832,7 @@ proof -
            apply (rotate_tac -2)
            apply (rule trans[rotated])
             apply (erule arg_cong)
-           apply (subst FFVars_vvsubstss)
+           apply (subst FVars_vvsubstss)
               apply (rule supp_id_bound bij_id)+
            apply (rule image_id[symmetric])
           (* END REPEAT_DETERM *)
@@ -4887,7 +4920,7 @@ proof -
               apply (erule arg_cong)
              apply (rule sym)
              apply (rule trans)
-              apply (rule FFVars_vvsubstss)
+              apply (rule FVars_vvsubstss)
                 apply (rule supp_id_bound bij_id)+
              apply (rule image_id)
         (* repeated *)
@@ -4911,7 +4944,7 @@ proof -
               apply (erule arg_cong)
              apply (rule sym)
              apply (rule trans)
-              apply (rule FFVars_vvsubstss)
+              apply (rule FVars_vvsubstss)
                 apply (rule supp_id_bound bij_id)+
             apply (rule image_id)
           (* END REPEAT_DETERM *)
@@ -4938,7 +4971,7 @@ proof -
               apply (erule arg_cong)
              apply (rule sym)
              apply (rule trans)
-              apply (rule FFVars_vvsubstss)
+              apply (rule FVars_vvsubstss)
                 apply (rule supp_id_bound bij_id)+
           apply (rule image_id)
         (* repeated *)
@@ -4963,7 +4996,7 @@ proof -
               apply (erule arg_cong)
              apply (rule sym)
              apply (rule trans)
-              apply (rule FFVars_vvsubstss)
+              apply (rule FVars_vvsubstss)
                 apply (rule supp_id_bound bij_id)+
           apply (rule image_id)
         (* repeated *)
@@ -4987,7 +5020,7 @@ proof -
               apply (erule arg_cong)
              apply (rule sym)
              apply (rule trans)
-              apply (rule FFVars_vvsubstss)
+              apply (rule FVars_vvsubstss)
                 apply (rule supp_id_bound bij_id)+
           apply (rule image_id)
         (* END REPEAT_DETERM *)
@@ -5063,7 +5096,7 @@ proof -
         (* END REPEAT twice *)
        apply (rule rel_T1_rel_T2.intros)
              apply (rule bij_id supp_id_bound id_on_id)+
-       apply (unfold T1.rrename_id0s T1_pre.map_id)
+       apply (unfold T1.permute_id0s T1_pre.map_id)
        apply (subst T1_pre.map_comp[OF assms, of id id id id id id id _ _ _ _ _ id id id id id, unfolded id_o o_id, symmetric])
             apply (rule supp_id_bound bij_id)+
        apply (subst (2) T1_pre.map_comp[OF assms, of id id id id id id id _ _ _ _ _ id id id id id, unfolded id_o o_id, symmetric])
@@ -5162,7 +5195,7 @@ proof -
         (* END REPEAT twice *)
       apply (rule rel_T1_rel_T2.intros)
             apply (rule bij_id supp_id_bound id_on_id)+
-      apply (unfold T1.rrename_id0s T2_pre.map_id)
+      apply (unfold T1.permute_id0s T2_pre.map_id)
       apply (subst T2_pre.map_comp[OF assms, of id id id id id id id _ _ _ _ _ id id id id id, unfolded id_o o_id, symmetric])
            apply (rule supp_id_bound bij_id)+
       apply (subst (2) T2_pre.map_comp[OF assms, of id id id id id id id _ _ _ _ _ id id id id id, unfolded id_o o_id, symmetric])
@@ -5278,8 +5311,8 @@ subclass (in var_T1) var_T2_pre
 mrbnf "('var, 'tyvar, 'a, 'b) T1"
   map: vvsubst_T1
   sets:
-    free: FFVars_T11
-    free: FFVars_T12
+    free: FVars_T11
+    free: FVars_T12
     free: set3_T1
     live: set4_T1
   bd: natLeq
@@ -5290,13 +5323,13 @@ mrbnf "('var, 'tyvar, 'a, 'b) T1"
     apply (rule trans)
      apply (rule vvsubst_rrenames)
         apply (rule supp_id_bound bij_id)+
-    apply (rule T1.rrename_id0s)
+    apply (rule T1.permute_id0s)
     done
               apply (rule vvsubst_comp0s; assumption)
              apply (rule vvsubst_cong; assumption)
-            apply (rule ext, (unfold comp_def)[1], rule FFVars_vvsubstss set3_map set4_map; assumption)+
+            apply (rule ext, (unfold comp_def)[1], rule FVars_vvsubstss set3_map set4_map; assumption)+
         apply (rule infinite_regular_card_order_natLeq)
-       apply (rule T1.FFVars_bd)+
+       apply (rule T1.FVars_bd)+
      apply (rule set_bd)+
    apply (rule rel_OO_mono)
   apply (rule iffI)
@@ -5311,8 +5344,8 @@ mrbnf "('var, 'tyvar, 'a, 'b) T1"
 mrbnf "('var, 'tyvar, 'a, 'b) T2"
   map: vvsubst_T2
   sets:
-    free: FFVars_T21
-    free: FFVars_T22
+    free: FVars_T21
+    free: FVars_T22
     free: set3_T2
     live: set4_T2
   bd: natLeq
@@ -5323,13 +5356,13 @@ mrbnf "('var, 'tyvar, 'a, 'b) T2"
     apply (rule trans)
      apply (rule vvsubst_rrenames)
         apply (rule supp_id_bound bij_id)+
-    apply (rule T1.rrename_id0s)
+    apply (rule T1.permute_id0s)
     done
               apply (rule vvsubst_comp0s; assumption)
              apply (rule vvsubst_cong; assumption)
-            apply (rule ext, (unfold comp_def)[1], rule FFVars_vvsubstss set3_map set4_map; assumption)+
+            apply (rule ext, (unfold comp_def)[1], rule FVars_vvsubstss set3_map set4_map; assumption)+
         apply (rule infinite_regular_card_order_natLeq)
-       apply (rule T1.FFVars_bd)+
+       apply (rule T1.FVars_bd)+
      apply (rule set_bd)+
    apply (rule rel_OO_mono)
   apply (rule iffI)
